New, hopefully sound release-acquire rules.

mailbox/acq_rel_atomics.v
@@ -1,4 +1,5 @@
 Require Import veric.rmaps.
+Require Import veric.compcert_rmaps.
 Require Import progs.conclib.
 Require Import progs.ghost.
 Require Import floyd.library.
@@ -98,29 +99,35 @@ Proof.
   apply derives_view_shift; Exists x x; auto.
 Qed.
 
-Lemma duplicable_super_non_expansive : forall n P, compcert_rmaps.RML.R.approx n (!!duplicable P) =
-  compcert_rmaps.RML.R.approx n (!!duplicable (compcert_rmaps.RML.R.approx n P)).
+Lemma duplicable_super_non_expansive : forall n P,
+  approx n (!!duplicable P) = approx n (!!duplicable (approx n P)).
 Proof.
   intros; unfold duplicable.
-  rewrite view_shift_super_non_expansive, approx_sepcon; auto.
+  setoid_rewrite view_shift_super_non_expansive at 1; rewrite approx_sepcon; auto.
 Qed.
 
 Section protocols.
 
 Context {state : Type}.
 
-(* Iris-weak gives a more in-depth encoding of protocol assertions in terms of invariants and ghost state. This
-   simpler one is probably still sound and almost as powerful. *)
+Class protocol {state : Type} (Iread Ifull : state -> Z -> mpred) :=
+  { full_read s v : view_shift (Ifull s v) (Ifull s v * Iread s v); read_dup s v : duplicable (Iread s v) }.
+
+(* Iris-weak gives an encoding of protocol assertions in terms of invariants, ghost state, and views. This
+   simpler one is unsound (because it is provably objective), but gives the right general feel.
 Definition protocol_inv (ord : state -> state -> Prop) T l g := EX v : Z, EX s : state,
   !!(repable_signed v) && data_at Tsh tint (vint v) l * ghost (gsh1, s) g * T s v.
 
 Definition protocol_piece (sh : share) l g (s : state) ord T :=
-  invariant (protocol_inv ord T l g) * ghost (sh, s) g.
+  invariant (protocol_inv ord T l g) * ghost (sh, s) g.*)
+
+Parameter protocol_piece : share -> val -> state -> (state -> state -> Prop) ->
+  ((state -> Z -> mpred) * (state -> Z -> mpred)) -> mpred.
 
 Definition protocol_R := protocol_piece Share.bot.
 Definition protocol_W := protocol_piece gsh2.
 
-Lemma protocol_inv_super_non_expansive : forall n ord T l g,
+(*Lemma protocol_inv_super_non_expansive : forall n ord T l g,
   compcert_rmaps.RML.R.approx n (protocol_inv ord T l g) =
   compcert_rmaps.RML.R.approx n (protocol_inv ord (fun s v => compcert_rmaps.RML.R.approx n (T s v)) l g).
 Proof.
@@ -128,223 +135,169 @@ Proof.
   rewrite !approx_exp; apply f_equal; extensionality v.
   rewrite !approx_exp; apply f_equal; extensionality s.
   rewrite !approx_sepcon, !approx_andp, approx_idem; auto.
-Qed.
+Qed.*)
 
-Lemma protocol_piece_super_non_expansive : forall n sh l g s ord T,
-  compcert_rmaps.RML.R.approx n (protocol_piece sh l g s ord T) =
-  compcert_rmaps.RML.R.approx n (protocol_piece sh l g s ord (fun s v => compcert_rmaps.RML.R.approx n (T s v))).
+Context `{PCM_order state} (Tread Tfull : state -> Z -> mpred).
+
+Axiom protocol_piece_nonexpansive : forall sh l s ord Tread1 Tfull1 Tread2 Tfull2,
+  (ALL s : state, ALL v : Z, (Tread1 s v <=> Tread2 s v) && (Tfull1 s v <=> Tfull2 s v)) |--
+  protocol_piece sh l s ord (Tread1, Tfull1) <=> protocol_piece sh l s ord (Tread2, Tfull2).
+
+Lemma protocol_piece_super_non_expansive : forall n sh l s ord Tread Tfull,
+  approx n (protocol_piece sh l s ord (Tread, Tfull)) =
+  approx n (protocol_piece sh l s ord (fun s v => approx n (Tread s v), fun s v => approx n (Tfull s v))).
 Proof.
-  intros; unfold protocol_piece.
-  rewrite !approx_sepcon; f_equal.
-  rewrite invariant_super_non_expansive; setoid_rewrite invariant_super_non_expansive at 2.
-  rewrite protocol_inv_super_non_expansive; auto.
+  intros.
+  apply approx_eq_i'.
+  intros m ?.
+  apply protocol_piece_nonexpansive.
+  intros ??; split; apply fash_equiv_approx; auto.
 Qed.
 
-Context `{PCM_order state}.
+Notation T := (Tread, Tfull).
 
-Lemma make_protocol_R : forall sh l g s T,
-  view_shift (protocol_piece sh l g s ord T) (protocol_piece sh l g s ord T * protocol_R l g s ord T).
-Proof.
-  intros; unfold protocol_W, protocol_R, protocol_piece.
-  rewrite <- sepcon_assoc, (sepcon_comm _ (invariant _)), <- sepcon_assoc, <- general_atomics.invariant_duplicable.
-  rewrite sepcon_assoc, !(sepcon_comm (invariant _)); apply invariant_view_shift.
-  unfold protocol_inv.
-  etransitivity; [apply view_shift_sepcon1, make_snap|].
-  rewrite (sepcon_comm _ (ghost _ _)); reflexivity.
-Qed.
+Axiom make_protocol_R : forall sh l s,
+  view_shift (protocol_piece sh l s ord T) (protocol_piece sh l s ord T * protocol_R l s ord T).
 
-Corollary protocol_R_duplicable : forall l g s T, duplicable (protocol_R l g s ord T).
-Proof.
-  intros; apply make_protocol_R.
-Qed.
-
-Corollary protocol_W_R : forall l g s T,
-  view_shift (protocol_W l g s ord T) (protocol_W l g s ord T * protocol_R l g s ord T).
+Corollary protocol_R_duplicable : forall l s, duplicable (protocol_R l s ord T).
 Proof.
   intros; apply make_protocol_R.
 Qed.
 
-Lemma protocol_R_absorb : forall sh l g s s' T, sh <> Share.bot ->
-  view_shift (protocol_piece sh l g s ord T * protocol_R l g s' ord T) (!!(ord s' s) && protocol_piece sh l g s ord T).
+Corollary protocol_W_R : forall l s,
+  view_shift (protocol_W l s ord T) (protocol_W l s ord T * protocol_R l s ord T).
 Proof.
-  intros; unfold protocol_R, protocol_piece.
-  rewrite <- sepcon_assoc, (sepcon_comm _ (invariant _)), <- sepcon_assoc, <- general_atomics.invariant_duplicable.
-  rewrite <- sepcon_andp_prop.
-  rewrite sepcon_assoc, !(sepcon_comm (invariant _)); apply invariant_view_shift.
-  unfold protocol_inv.
-  rewrite !(later_exp' _ 0); view_shift_intro v.
-  rewrite !(later_exp' _ s); view_shift_intro s0.
-  rewrite (sepcon_comm _ (ghost _ _)); setoid_rewrite snap_master_join; auto.
-  apply derives_view_shift; Exists v; entailer!.
-  apply sepcon_derives; auto.
-  apply later_derives; Exists s0; entailer!.
+  intros; apply make_protocol_R.
 Qed.
 
-Corollary protocol_R_W : forall l g s s' T,
-  view_shift (protocol_W l g s ord T * protocol_R l g s' ord T) (!!(ord s' s) && protocol_W l g s ord T).
+Axiom protocol_R_absorb : forall sh l s s', sh <> Share.bot ->
+  view_shift (protocol_piece sh l s ord T * protocol_R l s' ord T) (!!(ord s' s) && protocol_piece sh l s ord T).
+
+Corollary protocol_R_W : forall l s s',
+  view_shift (protocol_W l s ord T * protocol_R l s' ord T) (!!(ord s' s) && protocol_W l s ord T).
 Proof.
-  intros; apply protocol_R_absorb.
-  intro X; contradiction unreadable_bot; rewrite <- X; auto.
+  intros; apply protocol_R_absorb; auto.
 Qed.
 
-Lemma protocol_R_join : forall l g s1 s2 s T, join s1 s2 s ->
-  protocol_R l g s1 ord T * protocol_R l g s2 ord T = protocol_R l g s ord T.
-Proof.
-  intros; unfold protocol_R, protocol_piece.
-  rewrite <- sepcon_assoc, (sepcon_comm _ (invariant _)), <- sepcon_assoc, <- general_atomics.invariant_duplicable.
-  rewrite sepcon_assoc; setoid_rewrite ghost_snap_join; eauto; reflexivity.
-Qed.
+Axiom protocol_R_join : forall l s1 s2 s, join s1 s2 s ->
+  protocol_R l s1 ord T * protocol_R l s2 ord T = protocol_R l s ord T.
 
-Corollary protocol_R_R : forall l g s1 s2 T, ord s1 s2 ->
-  protocol_R l g s1 ord T * protocol_R l g s2 ord T = protocol_R l g s2 ord T.
+Corollary protocol_R_R : forall l s1 s2, ord s1 s2 ->
+  protocol_R l s1 ord T * protocol_R l s2 ord T = protocol_R l s2 ord T.
 Proof.
   intros; apply protocol_R_join.
   apply join_comm, ord_join; auto.
 Qed.
 
-Lemma protocol_R_join' : forall l g s1 s2 T,
-  protocol_R l g s1 ord T * protocol_R l g s2 ord T |--
-  EX s : _, !!(join s1 s2 s) && protocol_R l g s ord T.
+Axiom protocol_R_join' : forall l s1 s2,
+  protocol_R l s1 ord T * protocol_R l s2 ord T |--
+  EX s : _, !!(join s1 s2 s) && protocol_R l s ord T.
+
+Axiom make_protocol : forall {P : protocol Tread Tfull} l v s, repable_signed v ->
+  view_shift (data_at Tsh tint (vint v) l * Tfull s v) (protocol_W l s ord T).
+
+Axiom protocol_R_forget : forall l s1 s2, ord s1 s2 ->
+  view_shift (protocol_R l s2 ord T) (protocol_R l s1 ord T).
+
+Corollary protocol_R_choose : forall l s1 s2,
+  view_shift (protocol_R l s1 ord T * protocol_R l s2 ord T) (protocol_R l s1 ord T).
 Proof.
   intros.
-  assert_PROP (joins s1 s2) as Hs;
-    [|destruct Hs as (s & ?); Exists s; entailer!; erewrite protocol_R_join; eauto].
-  unfold protocol_R, protocol_piece; rewrite <- sepcon_assoc, (sepcon_comm _ (invariant _)), <- sepcon_assoc,
-    <- general_atomics.invariant_duplicable, sepcon_assoc, sepcon_comm.
-  apply sepcon_derives_prop.
-  eapply derives_trans; [apply ghost_conflict|].
-  apply prop_left; intros ((s', ?) & ? & Hjoin); simpl in *; apply prop_right.
-  rewrite !eq_dec_refl in Hjoin; eexists; eauto.
+  etransitivity; [apply derives_view_shift, protocol_R_join'|].
+  view_shift_intro s; view_shift_intros.
+  match goal with H : join _ _ _ |- _ => apply join_ord in H; destruct H end.
+  apply protocol_R_forget; auto.
 Qed.
 
-Lemma make_protocol' : forall l g v s T, repable_signed v ->
-  view_shift (data_at Tsh tint (vint v) l * ghost_master s g * T s v) (protocol_W l g s ord T).
-Proof.
-  intros.
-  setoid_rewrite <- ghost_var_share_join; eauto.
-  unfold protocol_W.
-  rewrite !sepcon_assoc, (sepcon_comm (ghost_var gsh2 _ _)), <- !sepcon_assoc.
-  apply view_shift_sepcon1, make_inv.
-  unfold protocol_inv.
-  Exists v s; entailer!.
-Qed.
-
-Lemma make_protocol : forall l v s T, repable_signed v ->
-  view_shift (data_at Tsh tint (vint v) l * T s v) (EX g : val, protocol_W l g s ord T).
-Proof.
-  intros.
-  etransitivity; [apply ghost_alloc with (g := (Tsh, s)), master_init|].
-  view_shift_intro g; etransitivity; [etransitivity; [|apply make_protocol'; eauto]|].
-  - apply derives_view_shift; cancel.
-  - apply derives_view_shift; Exists g; auto.
-Qed.
-
-Lemma protocol_R_forget : forall l g s1 s2 T
-  (Hcompat : forall s' s'', ord s1 s2 -> join s2 s' s'' -> exists s0, join s1 s' s0 /\ ord s0 s''),
-  ord s1 s2 -> view_shift (protocol_R l g s2 ord T) (protocol_R l g s1 ord T).
-Proof.
-  intros; unfold protocol_R.
-  apply view_shift_sepcon2, ghost_snap_forget; auto.
-Qed.
-
-Lemma protocol_R_choose : forall l g s1 s2 T
-  (Hcompat : forall s2 s' s'', ord s1 s2 -> join s2 s' s'' -> exists s0, join s1 s' s0 /\ ord s0 s''),
-  view_shift (protocol_R l g s1 ord T * protocol_R l g s2 ord T) (protocol_R l g s1 ord T).
-Proof.
-  intros; unfold protocol_R, protocol_piece.
-  rewrite <- sepcon_assoc, (sepcon_comm _ (invariant _)), <- sepcon_assoc, <- general_atomics.invariant_duplicable.
-  rewrite sepcon_assoc; apply view_shift_sepcon2, ghost_snap_choose; auto.
-Qed.
-
-Lemma protocol_piece_share_join : forall sh1 sh2 sh l g s1 s2 T (Hsh : sepalg.join sh1 sh2 sh)
+Axiom protocol_piece_share_join : forall sh1 sh2 sh l s1 s2 (Hsh : sepalg.join sh1 sh2 sh)
   (Hsh1 : readable_share sh1) (Hsh2 : readable_share sh2),
-  protocol_piece sh1 l g s1 ord T * protocol_piece sh2 l g s2 ord T =
-  !!(s1 = s2) && protocol_piece sh l g s1 ord T.
-Proof.
-  intros; unfold protocol_piece.
-  rewrite <- sepcon_assoc, (sepcon_comm _ (invariant _)), <- sepcon_assoc, <- general_atomics.invariant_duplicable.
-  rewrite sepcon_assoc; setoid_rewrite ghost_var_share_join'; eauto.
-  apply mpred_ext; entailer!.
-Qed.
+  protocol_piece sh1 l s1 ord T * protocol_piece sh2 l s2 ord T =
+  !!(s1 = s2) && protocol_piece sh l s1 ord T.
 
 End protocols.
-
-Existing Instance max_PCM.
-
-Lemma protocol_R_choose' : forall l g s1 s2 T,
-  view_shift (protocol_R l g s1 Z.le T * protocol_R l g s2 Z.le T) (protocol_R l g s1 Z.le T).
-Proof.
-  intros; apply protocol_R_choose; simpl; intros; subst.
-  do 2 eexists; eauto; apply Z.max_le_compat_r; auto.
-Qed.
 
 Definition OrdType s := ArrowType s (ArrowType s (ConstType Prop)).
 Definition PredType s := ArrowType s (ArrowType (ConstType Z) Mpred).
 
-Definition LA_type := ProdType (ProdType (ProdType (ProdType (ProdType (ConstType (val * val))
-  (DependentType 0)) (OrdType (DependentType 0))) (PredType (DependentType 0))) Mpred)
-  (PredType (DependentType 0)).
+Definition LA_type := ProdType (ProdType (ProdType (ProdType (ProdType (ProdType (ProdType (ProdType
+  (ConstType val) (DependentType 0)) (OrdType (DependentType 0)))
+  (ProdType (PredType (DependentType 0)) (PredType (DependentType 0))))
+  Mpred) (ArrowType (ConstType Z) Mpred)) (ConstType (list Z))) Mpred) (PredType (DependentType 0)).
 
 Program Definition load_acq_spec := TYPE LA_type
-  WITH l : val, g : val, s : _, ord : _ -> _ -> Prop, T : _ -> Z -> mpred, P : mpred, Q : _ -> Z -> mpred
+  WITH l : val, s : _, st_ord : _ -> _ -> Prop, T : ((_ -> Z -> mpred) * (_ -> Z -> mpred)),
+       P : mpred, II : Z -> mpred, lI : list Z, P' : mpred, Q : _ -> Z -> mpred
   PRE [ 1%positive OF tptr tint ]
-   PROP (forall s' v, ord s s' -> repable_signed v -> view_shift (P * T s' v) (P * T s' v * Q s' v)%logic;
-         forall s' v, duplicable (Q s' v))
+   PROP (view_shift (fold_right sepcon emp (map (fun p => |>II p) lI) * P)
+                    (protocol_R l s st_ord T * P');
+         forall s' v, st_ord s s' -> repable_signed v ->
+           view_shift (fst T s' v * protocol_R l s' st_ord T * P')%logic
+           (fold_right sepcon emp (map (fun p => |>II p) lI) * Q s' v))
    LOCAL (temp 1%positive l)
-   SEP (protocol_R l g s ord T; P)
+   SEP (fold_right sepcon emp (map (fun p => invariant (II p)) lI); P)
   POST [ tint ]
    EX v : Z, EX s' : _,
-   PROP (repable_signed v; ord s s')
+   PROP (repable_signed v; st_ord s s')
    LOCAL (temp ret_temp (vint v))
-   SEP (protocol_R l g s' ord T; P; Q s' v).
+   SEP (fold_right sepcon emp (map (fun p => invariant (II p)) lI); Q s' v).
 Next Obligation.
 Proof.
   repeat intro.
-  destruct x as ((((((?, ?), s), ?), ?), ?), ?); simpl.
+  destruct x as ((((((((?, s), ?), (?, ?)), P), ?), ?), ?), Q); simpl.
   unfold PROPx; simpl; rewrite !approx_andp; f_equal.
-  - rewrite !prop_and, !approx_andp; f_equal.
+  - rewrite !prop_and, !approx_andp; f_equal; [|f_equal].
+    + rewrite view_shift_super_non_expansive.
+      setoid_rewrite view_shift_super_non_expansive at 2; do 2 apply f_equal; f_equal.
+      * rewrite !approx_sepcon, !approx_sepcon_list', approx_idem.
+        erewrite !map_map, map_ext; eauto.
+        intro; simpl; rewrite nonexpansive_super_non_expansive by (apply later_nonexpansive); auto.
+      * unfold protocol_R; rewrite !approx_sepcon, approx_idem, protocol_piece_super_non_expansive; auto.
     + rewrite !prop_forall, !(approx_allp _ _ _ s); f_equal; extensionality s'.
       rewrite !prop_forall, !(approx_allp _ _ _ 0); f_equal; extensionality v'.
       rewrite !prop_impl; setoid_rewrite approx_imp; do 2 apply f_equal.
       setoid_rewrite approx_imp; do 2 apply f_equal.
-      rewrite view_shift_super_non_expansive, !approx_sepcon; auto.
-    + f_equal.
-      rewrite !prop_forall, !(approx_allp _ _ _ s); f_equal; extensionality s'.
-      rewrite !prop_forall, !(approx_allp _ _ _ 0); f_equal; extensionality v'.
-      apply duplicable_super_non_expansive.
+      rewrite view_shift_super_non_expansive.
+      setoid_rewrite view_shift_super_non_expansive at 2.
+      unfold protocol_R; rewrite !approx_sepcon, !approx_sepcon_list', protocol_piece_super_non_expansive, !approx_idem.
+      erewrite !map_map, map_ext; eauto.
+      intro; simpl; rewrite nonexpansive_super_non_expansive by (apply later_nonexpansive); auto.
   - unfold LOCALx; simpl; rewrite !approx_andp; apply f_equal.
-    unfold SEPx, protocol_R; simpl; rewrite !approx_sepcon, protocol_piece_super_non_expansive, approx_idem; auto.
+    unfold SEPx; simpl; rewrite !sepcon_emp, !approx_sepcon, !approx_idem, !approx_sepcon_list'.
+    erewrite !map_map, map_ext; eauto.
+    intros; simpl; rewrite invariant_super_non_expansive; auto.
 Qed.
 Next Obligation.
 Proof.
   repeat intro.
-  destruct x as ((((((?, ?), ?), ?), ?), ?), ?); simpl.
-  rewrite !approx_exp; apply f_equal; extensionality vr.
+  destruct x as ((((((((?, ?), ?), ?), ?), ?), ?), ?), ?); simpl.
+  rewrite !approx_exp; apply f_equal; extensionality v'.
   rewrite !approx_exp; apply f_equal; extensionality s'.
-  unfold PROPx; simpl; rewrite !approx_andp; apply f_equal.
-  unfold LOCALx; simpl; rewrite !approx_andp; apply f_equal.
-  unfold SEPx, protocol_R; simpl; rewrite !approx_sepcon, protocol_piece_super_non_expansive, !approx_idem; auto.
+  unfold PROPx, LOCALx, SEPx; simpl; rewrite !approx_andp; do 2 apply f_equal;
+    rewrite !sepcon_emp, ?approx_sepcon, ?approx_idem.
+  rewrite !approx_sepcon_list'.
+  erewrite !map_map, map_ext; eauto.
+  intros; simpl; rewrite invariant_super_non_expansive; auto.
 Qed.
 
 Definition SR_type := ProdType (ProdType (ProdType (ProdType (ProdType (ProdType (ProdType (ProdType (ProdType
-  (ConstType (val * Z * val)) (DependentType 0)) (DependentType 0)) (OrdType (DependentType 0))) (PredType (DependentType 0)))
+  (ConstType (val * Z)) (DependentType 0)) (DependentType 0)) (OrdType (DependentType 0)))
+  (ProdType (PredType (DependentType 0)) (PredType (DependentType 0))))
   Mpred) (ArrowType (ConstType Z) Mpred)) (ConstType (list Z))) Mpred) Mpred.
 
 (* single_writer version - multi-writer version uses protocol_R and requires that for all s',
    ord s s' -> ord s' s''. *)
 (* Using the stronger version from iGPS that allows the writer to pass its own protocol_W assertion into the
    protocol invariant. *)
-(* Hypothesis: in the single-writer case, it's sound to allow the writer to interact with invariants. *)
 Program Definition store_rel_spec := TYPE SR_type
-  WITH l : val, v : Z, g : val, s : _, s'' : _, st_ord : _ -> _ -> Prop, T : _ -> Z -> mpred,
+  WITH l : val, v : Z, s : _, s'' : _, st_ord : _ -> _ -> Prop, T : ((_ -> Z -> mpred) * (_ -> Z -> mpred)),
        P : mpred, II : Z -> mpred, lI : list Z, P' : mpred, Q : mpred
   PRE [ 1%positive OF tptr tint, 2%positive OF tint ]
    PROP (repable_signed v;
          view_shift (fold_right sepcon emp (map (fun p => |>II p) lI) * P)
-                    (protocol_W l g s st_ord T * P');
+                    (protocol_W l s st_ord T * P');
          forall v0, repable_signed v0 ->
-           view_shift (T s v0 * protocol_W l g s'' st_ord T * P')%logic
-           (T s'' v * fold_right sepcon emp (map (fun p => |>II p) lI) * Q)%logic; st_ord s s'')
+           view_shift (snd T s v0 * protocol_W l s'' st_ord T * P')%logic
+                      (snd T s'' v * fold_right sepcon emp (map (fun p => |>II p) lI) * Q)%logic; st_ord s s'')
    LOCAL (temp 1%positive l; temp 2%positive (vint v))
    SEP (fold_right sepcon emp (map (fun p => invariant (II p)) lI); P)
   POST [ tvoid ]
@@ -354,7 +307,7 @@ Program Definition store_rel_spec := TYPE SR_type
 Next Obligation.
 Proof.
   repeat intro.
-  destruct x as (((((((((((?, ?), ?), ?), ?), ?), ?), ?), ?), ?), ?), ?); simpl.
+  destruct x as ((((((((((?, ?), ?), ?), ?), (?, ?)), ?), ?), ?), ?), ?); simpl.
   unfold PROPx; simpl; rewrite !approx_andp; f_equal.
   - rewrite !prop_and, !approx_andp; f_equal; f_equal; [|f_equal].
     + rewrite view_shift_super_non_expansive.
@@ -378,7 +331,7 @@ Qed.
 Next Obligation.
 Proof.
   repeat intro.
-  destruct x as (((((((((((?, ?), ?), ?), ?), ?), ?), ?), ?), ?), ?), ?); simpl.
+  destruct x as ((((((((((?, ?), ?), ?), ?), ?), ?), ?), ?), ?), ?); simpl.
   unfold PROPx, LOCALx, SEPx; simpl; rewrite !approx_andp; do 2 apply f_equal;
     rewrite !sepcon_emp, ?approx_sepcon, ?approx_idem.
   rewrite !approx_sepcon_list'.
@@ -386,45 +339,71 @@ Proof.
   intros; simpl; rewrite invariant_super_non_expansive; auto.
 Qed.
 
-Definition CRA_type := ProdType (ProdType (ProdType (ProdType (ProdType (ProdType (ConstType (val * Z * Z * val))
+(*Definition CRA_type := ProdType (ProdType (ProdType (ProdType (ProdType (ProdType (ProdType (ProdType (ProdType
+  (ProdType (ConstType (val * Z * Z))
   (DependentType 0)) (DependentType 0)) (OrdType (DependentType 0))) (PredType (DependentType 0))) Mpred)
+  (ArrowType (ConstType Z) Mpred)) (ConstType (list Z))) Mpred) (ArrowType (ConstType Z) Mpred))
   (ArrowType (ConstType Z) Mpred).
 
 Program Definition CAS_RA_spec := TYPE CRA_type
-  WITH l : val, c : Z, v : Z, g : val, s : _, s'' : _, ord : _ -> _ -> Prop, T : _ -> Z -> mpred,
-       P : mpred, Q : Z -> mpred
+  WITH l : val, c : Z, v : Z, s : _, s'' : _, st_ord : _ -> _ -> Prop, T : _ -> Z -> mpred, P : mpred,
+       II : Z -> mpred, lI : list Z, P' : mpred, Q' : Z -> mpred, Q : Z -> mpred
   PRE [ 1%positive OF tptr tint, 2%positive OF tint, 3%positive OF tint ]
-   PROP (repable_signed c; repable_signed v; forall v0, repable_signed v0 ->
-     view_shift (P * T s v0) ((if eq_dec v0 c then T s'' v else T s v0) * Q v0); ord s s'')
+   PROP (repable_signed c; repable_signed v;
+         view_shift (fold_right sepcon emp (map (fun p => |>II p) lI) * P)
+                    (protocol_W l s st_ord T * P');
+         forall v0, repable_signed v0 ->
+           view_shift (P' * T s v0) ((if eq_dec v0 c then T s'' v else T s v0) * Q' v0);
+         forall v0, repable_signed v0 ->
+           view_shift (protocol_W l (if eq_dec v0 c then s'' else s) st_ord T * Q' v0)
+                      (fold_right sepcon emp (map (fun p => |>II p) lI) * Q v0); st_ord s s'')
    LOCAL (temp 1%positive l; temp 2%positive (vint c); temp 3%positive (vint v))
-   SEP (protocol_W l g s ord T; P)
+   SEP (fold_right sepcon emp (map (fun p => invariant (II p)) lI); P)
   POST [ tint ]
    EX v' : Z,
    PROP (repable_signed v')
    LOCAL (temp ret_temp (Val.of_bool (if eq_dec v' c then true else false)))
-   SEP (protocol_W l g (if eq_dec v' c then s'' else s) ord T; Q v').
+   SEP (fold_right sepcon emp (map (fun p => invariant (II p)) lI); Q v').
 Next Obligation.
 Proof.
   repeat intro.
-  destruct x as (((((((((?, ?), ?), ?), ?), ?), ?), ?), ?), ?); simpl.
+  destruct x as ((((((((((((?, ?), ?), ?), ?), ?), ?), ?), ?), ?), ?), ?), ?); simpl.
   unfold PROPx; simpl; rewrite !approx_andp; f_equal.
-  - rewrite !prop_and, !approx_andp; do 2 apply f_equal; f_equal.
-    rewrite !prop_forall, !(approx_allp _ _ _ 0); f_equal; extensionality v'.
-    rewrite !prop_impl; setoid_rewrite approx_imp; do 2 apply f_equal.
-    rewrite view_shift_super_non_expansive, !approx_sepcon; if_tac; auto.
+  - rewrite !prop_and, !approx_andp; do 2 apply f_equal; f_equal; [|f_equal].
+    + rewrite view_shift_super_non_expansive.
+      setoid_rewrite view_shift_super_non_expansive at 2; do 2 apply f_equal; f_equal.
+      * rewrite !approx_sepcon, !approx_sepcon_list', approx_idem.
+        erewrite !map_map, map_ext; eauto.
+        intro; simpl; rewrite nonexpansive_super_non_expansive by (apply later_nonexpansive); auto.
+      * unfold protocol_W; rewrite !approx_sepcon, approx_idem, protocol_piece_super_non_expansive; auto.
+    + rewrite !prop_forall, !(approx_allp _ _ _ 0); f_equal; extensionality v'.
+      rewrite !prop_impl; setoid_rewrite approx_imp; do 2 apply f_equal.
+      rewrite view_shift_super_non_expansive, !approx_sepcon; if_tac; auto.
+    + f_equal.
+      rewrite !prop_forall, !(approx_allp _ _ _ 0); f_equal; extensionality v'.
+      rewrite !prop_impl; setoid_rewrite approx_imp; do 2 apply f_equal.
+      rewrite view_shift_super_non_expansive.
+      setoid_rewrite view_shift_super_non_expansive at 2; do 2 apply f_equal; f_equal.
+      * unfold protocol_W; rewrite !approx_sepcon, approx_idem, protocol_piece_super_non_expansive; auto.
+      * rewrite !approx_sepcon, !approx_sepcon_list', approx_idem.
+        erewrite !map_map, map_ext; eauto.
+        intro; simpl; rewrite nonexpansive_super_non_expansive by (apply later_nonexpansive); auto.
   - unfold LOCALx; simpl; rewrite !approx_andp; f_equal.
-    unfold SEPx, protocol_W; simpl.
-    rewrite !approx_sepcon, protocol_piece_super_non_expansive, approx_idem; auto.
+    unfold SEPx; simpl; rewrite !sepcon_emp, !approx_sepcon, !approx_idem, !approx_sepcon_list'.
+    erewrite !map_map, map_ext; eauto.
+    intros; simpl; rewrite invariant_super_non_expansive; auto.
 Qed.
 Next Obligation.
 Proof.
   repeat intro.
-  destruct x as (((((((((?, ?), ?), ?), ?), ?), ?), ?), ?), ?); simpl.
+  destruct x as ((((((((((((?, ?), ?), ?), ?), ?), ?), ?), ?), ?), ?), ?), ?); simpl.
   rewrite !approx_exp; apply f_equal; extensionality vr.
   unfold PROPx; simpl; rewrite !approx_andp; f_equal.
   unfold LOCALx; simpl; rewrite !approx_andp; f_equal.
-  unfold SEPx, protocol_W; simpl; rewrite !approx_sepcon, protocol_piece_super_non_expansive, approx_idem; auto.
-Qed.
+  unfold SEPx; simpl; rewrite !sepcon_emp, !approx_sepcon, !approx_idem, !approx_sepcon_list'.
+  erewrite !map_map, map_ext; eauto.
+  intros; simpl; rewrite invariant_super_non_expansive; auto.
+Qed.*)
 
 End atomics.
 
