mailbox/verif_kvnode_atomic_ra.v
@@ -42,43 +42,137 @@ Proof.
 Qed.
 
 (* Lexicographic ordering doesn't lead to a PCM (it's not associative), so we keep a full log of values. *)
-Definition data_T g s (v : Z) := EX ver : Z, !!(Z.even ver = true /\ log_latest s ver v) &&
-  ghost_snap (ver - 1) g.
 
-Definition node_entry sh log locs g lg i :=
-  protocol_piece sh (Znth i locs Vundef) (Znth i lg Vundef) log map_incl (data_T g).
+(* In this example, all the resources held in the protocols are snapshots, so the full and read interpretations
+   are equal. *)
 
-Definition version_T locs g lg g' (s v : Z) := !!(v = s) && EX L : _,
+(* This is a bit messy to allow the mutually recursive protocol interpretations. *)
+Definition data_T' version version_T s (v : Z) := EX ver : Z, !!(Z.even ver = true /\ log_latest s ver v) &&
+  protocol_R version (ver - 1) Z.le (version_T, version_T).
+
+Definition version_T_fun version locs g : (Z * Z -> mpred) -> (Z * Z -> mpred) :=
+  fun R '(s, v) => !!(v = s) && EX L : _,
   !!(exists vs, Zlength vs = size /\ log_latest L (if Z.even v then v else v - 1) vs) &&
-  fold_right sepcon emp (map (fun i => node_entry Share.bot (map_Znth i L 0) locs g lg i) (upto (Z.to_nat size))) *
-  ghost_snap L g'.
+  fold_right sepcon emp (map (fun i => protocol_R (Znth i locs Vundef) (map_Znth i L 0) map_incl
+    (data_T' version (fun s v => |>R (s, v)), data_T' version (fun s v => |>R (s, v)))) (upto (Z.to_nat size))) *
+  ghost_snap L g.
+
+Definition version_T' version locs g := HORec (version_T_fun version locs g).
+Definition version_T version locs g s v := version_T' version locs g (s, v).
+
+Definition data_T version locs g := data_T' version (|>version_T version locs g).
+
+Lemma version_T'_eq version locs g : version_T' version locs g =
+  version_T_fun version locs g (version_T' version locs g).
+Proof.
+  apply HORec_fold_unfold, prove_HOcontractive.
+  intros P1 P2 (s, v).
+  unfold version_T_fun.
+  apply subp_andp; [apply subp_refl|].
+  apply subp_exp; intro L.
+  apply subp_sepcon; [|apply subp_refl].
+  apply subp_andp; [apply subp_refl|].
+  pose proof (fold_right_sepcon_nonexpansive
+    (map (fun i => protocol_R (Znth i locs Vundef) (map_Znth i L 0) map_incl
+      (data_T' version (fun s v => |>P1 (s, v)), data_T' version (fun s v => |>P1 (s, v)))) (upto (Z.to_nat size)))
+    (map (fun i => protocol_R (Znth i locs Vundef) (map_Znth i L 0) map_incl
+      (data_T' version (fun s v => |>P2 (s, v)), data_T' version (fun s v => |>P2 (s, v)))) (upto (Z.to_nat size)))) as H.
+  rewrite fash_andp in H.
+  eapply derives_trans; [eapply derives_trans, H; [|rewrite !Zlength_map; auto] | apply andp_left1; auto].
+  apply allp_right; intro i.
+  destruct (zlt i 0); [rewrite !Znth_underflow by auto; apply eqp_refl|].
+  destruct (zlt i (Zlength (upto (Z.to_nat size))));
+    [|rewrite !Znth_overflow by (rewrite Zlength_map; auto); apply eqp_refl].
+  erewrite !Znth_map, !Znth_upto by (auto; rewrite Zlength_upto in *; omega).
+  eapply derives_trans, protocol_piece_nonexpansive.
+  apply allp_right; intro s1.
+  apply allp_right; intro v1.
+  unfold data_T'.
+  eapply derives_trans, andp_right, derives_refl; auto.
+  apply eqp_exp; intro ver.
+  apply eqp_andp; [apply eqp_refl|].
+  eapply derives_trans, protocol_piece_nonexpansive.
+  apply allp_right; intro s2.
+  apply allp_right; intro v2.
+  apply allp_left with (s2, v2), andp_right; apply derives_refl.
+Qed.
+
+Lemma version_T_eq version locs g s v : version_T version locs g s v = !!(v = s) && EX L : _,
+  !!(exists vs, Zlength vs = size /\ log_latest L (if Z.even v then v else v - 1) vs) &&
+  fold_right sepcon emp (map (fun i => protocol_R (Znth i locs Vundef) (map_Znth i L 0) map_incl
+    (data_T version locs g, data_T version locs g)) (upto (Z.to_nat size))) * ghost_snap L g.
+Proof.
+  intros; unfold version_T.
+  etransitivity; [rewrite version_T'_eq; reflexivity | auto].
+Qed.
+
+Lemma data_T_eq version locs g s v : data_T version locs g s v =
+  EX ver : Z, !!(Z.even ver = true /\ log_latest s ver v) &&
+    protocol_R version (ver - 1) Z.le (|>version_T version locs g, |>version_T version locs g).
+Proof. auto. Qed.
+
+(* up *)
+Global Instance dup_protocol {state} (T : state -> Z -> mpred) (Ht : forall s v, duplicable (T s v)) :
+  protocol T T.
+Proof.
+  split; auto.
+Qed.
+
+Existing Instance max_PCM.
+Existing Instance max_order.
+Existing Instance fmap_PCM.
+Existing Instance fmap_order.
+
+Lemma data_T_duplicable : forall version locs g s v, duplicable (data_T version locs g s v).
+Proof.
+  intros; rewrite data_T_eq.
+  apply exp_duplicable; intro.
+  apply prop_duplicable, protocol_R_duplicable.
+Qed.
+
+Instance data_prot version locs g : protocol (data_T version locs g) (data_T version locs g).
+Proof.
+  apply dup_protocol, data_T_duplicable.
+Qed.
+
+Lemma version_T_duplicable : forall version locs g s v, duplicable (version_T version locs g s v).
+Proof.
+  intros; rewrite version_T_eq.
+  apply prop_duplicable, exp_duplicable; intro.
+  apply sepcon_duplicable, ghost_snap_duplicable.
+  apply prop_duplicable, sepcon_list_duplicable.
+  rewrite Forall_map, Forall_forall; intros.
+  apply protocol_R_duplicable.
+Qed.
+
+Instance version_prot version locs g : protocol (version_T version locs g) (version_T version locs g).
+Proof.
+  apply dup_protocol, version_T_duplicable.
+Qed.
 
 (* The collection of protocol assertions that describes a stable state of the node. *)
-Definition node_state (sh : share) (L : Z -> option (list Z)) v version locs g lg g' :=
+Definition node_state (sh : share) (L : Z -> option (list Z)) v version locs g :=
   !!(Z.even v = true /\ exists vs, Zlength vs = size /\ log_latest L v vs) &&
-  protocol_piece sh version g v Z.le (version_T locs g lg g') *
-  fold_right sepcon emp (map (fun i => node_entry sh (map_Znth i L 0) locs g lg i) (upto (Z.to_nat size))) *
-  ghost (sh, L) g'.
-
-(* Posit a version in which protocol assertions cannot be stored in invariants under any circumstances. *)
+  protocol_piece sh version v Z.le (version_T version locs g, version_T version locs g) *
+  fold_right sepcon emp (map (fun i => protocol_piece sh (Znth i locs Vundef) (map_Znth i L 0) map_incl
+    (data_T version locs g, data_T version locs g)) (upto (Z.to_nat size))) * ghost (sh, L) g.
 
 Program Definition read_spec := DECLARE _read atomic_spec
-  (ConstType (val * val * share * share * val * list val * val * val * list val * (Z -> option (list Z)) * Z))
+  (ConstType (val * val * share * share * val * list val * val * (Z -> option (list Z)) * Z))
   empty_map [(_n, tptr tnode); (_out, tptr tint)] tvoid
-  [fun _ '(n, out, sh, shi, version, locs, g, g', lg, L0, v0) => temp _n n;
-   fun _ '(n, out, sh, shi, version, locs, g, g', lg, L0, v0) => temp _out out]
-  (fun _ '(n, out, sh, shi, version, locs, g, g', lg, L0, v0) => !!(readable_share sh /\
+  [fun _ '(n, out, sh, shi, version, locs, g, L0, v0) => temp _n n;
+   fun _ '(n, out, sh, shi, version, locs, g, L0, v0) => temp _out out]
+  (fun _ '(n, out, sh, shi, version, locs, g, L0, v0) => !!(readable_share sh /\
      writable_share shi /\ isptr version /\ Forall isptr locs /\ Zlength locs = size) &&
    data_at sh tnode (version, locs) n * data_at_ shi (tarray tint size) out *
-   node_state Share.bot L0 v0 version locs g lg g')
-  (fun _ '(n, out, sh, shi, version, locs, g, g', lg, L0, v0) L => ghost (gsh1, L) g')
+   node_state Share.bot L0 v0 version locs g)
+  (fun _ '(n, out, sh, shi, version, locs, g, L0, v0) L => ghost (gsh1, L) g)
   (0, []) []
-  (fun _ '(n, out, sh, shi, version, locs, g, g', lg, L0, v0) L '(v, vals) =>
+  (fun _ '(n, out, sh, shi, version, locs, g, L0, v0) L '(v, vals) =>
    !!(v0 <= v /\ Zlength vals = size /\ (v = v0 -> L0 v = Some vals)) &&
    data_at sh tnode (version, locs) n * data_at shi (tarray tint size) (map (fun x => vint x) vals) out *
-   node_state Share.bot (singleton v vals) v version locs g lg g')
-  (fun _ '(n, out, sh, shi, version, locs, g, g', lg, L0, v0) L '(v, vals) => !!(L v = Some vals) &&
-   ghost (gsh1, L) g')
+   node_state Share.bot (singleton v vals) v version locs g)
+  (fun _ '(n, out, sh, shi, version, locs, g, L0, v0) L '(v, vals) => !!(L v = Some vals) && ghost (gsh1, L) g)
   _ _ _ _ _ _.
 Next Obligation.
 Proof.
@@ -106,23 +200,21 @@ Proof.
 Qed.
 
 Program Definition write_spec := DECLARE _write atomic_spec
-  (ConstType (val * val * share * share * val * list val * list Z * val * val * list val *
-              (Z -> option (list Z)) * Z))
+  (ConstType (val * val * share * share * val * list val * list Z * val * (Z -> option (list Z)) * Z))
   (@empty_map Z (list Z)) [(_n, tptr tnode); (_in, tptr tint)] tvoid
-  [fun _ '(n, input, sh, shi, version, locs, vals, g, g', lg, L, v0) => temp _n n;
-   fun _ '(n, input, sh, shi, version, locs, vals, g, g', lg, L, v0) => temp _in input]
-  (fun _ '(n, input, sh, shi, version, locs, vals, g, g', lg, L, v0) => !!(readable_share sh /\
+  [fun _ '(n, input, sh, shi, version, locs, vals, g, L, v0) => temp _n n;
+   fun _ '(n, input, sh, shi, version, locs, vals, g, L, v0) => temp _in input]
+  (fun _ '(n, input, sh, shi, version, locs, vals, g, L, v0) => !!(readable_share sh /\
      readable_share shi /\ isptr version /\ Forall isptr locs /\ Zlength locs = size /\
      Forall repable_signed vals) &&
    data_at sh tnode (version, locs) n * data_at shi (tarray tint size) (map (fun x => vint x) vals) input *
-   node_state gsh2 L v0 version locs g lg g')
-  (fun _ '(n, input, sh, shi, version, locs, vals, g, g', lg, L, v0) L' => ghost (gsh1, L') g')
+   node_state gsh2 L v0 version locs g)
+  (fun _ '(n, input, sh, shi, version, locs, vals, g, L, v0) L' => ghost (gsh1, L') g)
   tt []
-  (fun _ '(n, input, sh, shi, version, locs, vals, g, g', lg, L, v0) _ _ =>
+  (fun _ '(n, input, sh, shi, version, locs, vals, g, L, v0) _ _ =>
    data_at sh tnode (version, locs) n * data_at shi (tarray tint size) (map (fun x => vint x) vals) input *
-   node_state gsh2 (map_upd L (v0 + 2) vals) (v0 + 2) version locs g lg g')
-  (fun _ '(n, input, sh, shi, version, locs, vals, g, g', lg, L, v0) _ _ =>
-   ghost (gsh1, map_upd L (v0 + 2) vals) g')
+   node_state gsh2 (map_upd L (v0 + 2) vals) (v0 + 2) version locs g)
+  (fun _ '(n, input, sh, shi, version, locs, vals, g, L, v0) _ _ => ghost (gsh1, map_upd L (v0 + 2) vals) g)
   _ _ _ _ _ _.
 Next Obligation.
 Proof.
@@ -156,28 +248,27 @@ Definition make_node_spec := DECLARE _make_node
     LOCAL ()
     SEP ()
   POST [ tptr tnode ]
-   EX n : val, EX version : val, EX locs : list val, EX g : val, EX lg : list val, EX g' : val,
+   EX n : val, EX version : val, EX locs : list val, EX g : val,
     PROP (isptr version; Forall isptr locs; Zlength locs = size)
     LOCAL (temp ret_temp n)
     SEP (data_at Tsh tnode (version, locs) n; malloc_token Tsh (sizeof tnode) n;
          malloc_token Tsh (sizeof tint) version; fold_right sepcon emp (map (malloc_token Tsh (sizeof tint)) locs);
-         node_state gsh2 (singleton 0 (repeat 0 (Z.to_nat size))) 0 version locs g lg g';
-         ghost (gsh1, singleton 0 (repeat 0 (Z.to_nat size))) g').
+         node_state gsh2 (singleton 0 (repeat 0 (Z.to_nat size))) 0 version locs g;
+         ghost (gsh1, singleton 0 (repeat 0 (Z.to_nat size))) g).
 
 Definition writer_spec := DECLARE _writer
-  WITH n : val, sh : share, v : Z, L : Z -> option (list Z), version : val, locs : list val,
-       g : val, lg : list val, g' : val
+  WITH n : val, sh : share, v : Z, L : Z -> option (list Z), version : val, locs : list val, g : val
   PRE [ _n OF tptr tvoid ]
     PROP (readable_share sh; isptr version; Forall isptr locs; Zlength locs = size)
     LOCAL (temp _n n)
-    SEP (data_at sh tnode (version, locs) n; node_state gsh2 L v version locs g lg g';
-         invariant (EX L : Z -> option (list Z), ghost (gsh1, L) g'))
+    SEP (data_at sh tnode (version, locs) n; node_state gsh2 L v version locs g;
+         invariant (EX L : Z -> option (list Z), ghost (gsh1, L) g))
   POST [ tptr tvoid ]
    EX L' : _,
     PROP (L' = map_upd_list L (map (fun i => (v + (2 * (i + 1)), repeat (i + 1) (Z.to_nat size)))%Z (upto 3)))
     LOCAL ()
-    SEP (data_at sh tnode (version, locs) n; node_state gsh2 L' (v + 6) version locs g lg g';
-         invariant (EX L : Z -> option (list Z), ghost (gsh1, L) g')).
+    SEP (data_at sh tnode (version, locs) n; node_state gsh2 L' (v + 6) version locs g;
+         invariant (EX L : Z -> option (list Z), ghost (gsh1, L) g)).
 
 (*Definition reader_spec := DECLARE _reader
   WITH n : val, sh : share, version : val, locs : list val, g : val, g' : val,
@@ -211,19 +302,18 @@ Definition writer_spec := DECLARE _writer
   _ _ _ _ _ _. (* We could encapsulate this with another argument to node_inv, a known sublist of hr. *)*)
 
 Definition reader_spec := DECLARE _reader
-  WITH n : val, sh : share, v : Z, L : Z -> option (list Z), version : val, locs : list val,
-       g : val, g' : val, lg : list val
+  WITH n : val, sh : share, v : Z, L : Z -> option (list Z), version : val, locs : list val, g : val
   PRE [ _n OF tptr tvoid ]
     PROP (readable_share sh; isptr version; Forall isptr locs; Zlength locs = size)
     LOCAL (temp _n n)
-    SEP (data_at sh tnode (version, locs) n; node_state Share.bot L v version locs g lg g';
-         invariant (EX L : Z -> option (list Z), ghost (gsh1, L) g'))
+    SEP (data_at sh tnode (version, locs) n; node_state Share.bot L v version locs g;
+         invariant (EX L : Z -> option (list Z), ghost (gsh1, L) g))
   POST [ tptr tvoid ]
    EX v' : Z, EX vs' : list Z,
     PROP (v <= v'; v' = v -> Z.even v = true /\ L v = Some vs')
     LOCAL ()
-    SEP (data_at sh tnode (version, locs) n; node_state Share.bot (map_upd L v' vs') v' version locs g lg g';
-         invariant (EX L : Z -> option (list Z), ghost (gsh1, L) g')).
+    SEP (data_at sh tnode (version, locs) n; node_state Share.bot (map_upd L v' vs') v' version locs g;
+         invariant (EX L : Z -> option (list Z), ghost (gsh1, L) g)).
 
 Definition Gprog : funspecs := ltac:(with_library prog [surely_malloc_spec; load_acq_spec; store_rel_spec;
   read_spec; write_spec; make_node_spec; writer_spec; reader_spec]).
@@ -251,21 +341,6 @@ Proof.
   intros; apply Z.land_ones with (n := 1); omega.
 Qed.
 
-Existing Instance max_PCM.
-Existing Instance max_order.
-Existing Instance fmap_PCM.
-Existing Instance fmap_order.
-
-Lemma version_T_duplicable : forall locs g lg g' s v, duplicable (version_T locs g lg g' s v).
-Proof.
-  intros; unfold version_T.
-  apply prop_duplicable, exp_duplicable; intro.
-  apply sepcon_duplicable, ghost_snap_duplicable.
-  apply prop_duplicable, sepcon_list_duplicable.
-  rewrite Forall_map, Forall_forall; intros; simpl.
-  unfold node_entry; apply protocol_R_duplicable.
-Qed.
-
 Definition list_max v l := fold_right Z.max v l.
 
 Lemma list_max_app : forall v l1 l2, list_max v (l1 ++ l2) = list_max (list_max v l2) l1.
@@ -290,26 +365,18 @@ Proof.
     + etransitivity; eauto; apply Zle_max_l.
 Qed.
 
-Lemma node_entry_single : forall log locs g lg i v v', log v = Some v' ->
-  view_shift (node_entry Share.bot log locs g lg i) (node_entry Share.bot (singleton v v') locs g lg i).
+Lemma protocol_R_single : forall version locs l log g v v', log v = Some v' ->
+  view_shift (protocol_R l log map_incl (data_T version locs g, data_T version locs g))
+             (protocol_R l (singleton v v') map_incl (data_T version locs g, data_T version locs g)).
 Proof.
-  intros; unfold node_entry.
-  apply protocol_R_forget with (s1 := singleton v v'); try apply map_join_incl_compat.
-  unfold singleton, map_Znth; intros ??; if_tac; [|discriminate].
+  intros; apply protocol_R_forget.
+  unfold singleton; intros ??; if_tac; [|discriminate].
   intro X; inv X; auto.
 Qed.
 
-Lemma node_entry_snap : forall sh log locs g lg i,
-  view_shift (node_entry sh log locs g lg i)
-    (node_entry sh log locs g lg i * node_entry Share.bot log locs g lg i).
-Proof.
-  intros; unfold node_entry.
-  apply make_protocol_R.
-Qed.
-
-Lemma node_state_snap : forall sh L v version locs g lg g',
-  view_shift (node_state sh L v version locs g lg g')
-    (node_state sh L v version locs g lg g' * node_state Share.bot L v version locs g lg g').
+Lemma node_state_snap : forall sh L v version locs g,
+  view_shift (node_state sh L v version locs g)
+             (node_state sh L v version locs g * node_state Share.bot L v version locs g).
 Proof.
   intros; unfold node_state; view_shift_intros.
   rewrite !sepcon_assoc.
@@ -320,34 +387,25 @@ Proof.
     { rewrite 2Zlength_map; reflexivity. }
     rewrite Zlength_map; intros.
     erewrite !Znth_map, !Znth_upto by (auto; rewrite Zlength_upto in *; omega).
-    apply node_entry_snap.
+    apply make_protocol_R.
   - rewrite sepcon_map.
     apply derives_view_shift; entailer!.
 Qed.
 
-Lemma node_entry_absorb : forall sh L1 L2 locs g lg i,
-  view_shift (node_entry sh L1 locs g lg i * node_entry Share.bot L2 locs g lg i)
-    (node_entry sh L1 locs g lg i).
-Proof.
-  intros.
-  destruct (eq_dec sh Share.bot).
-  - subst; apply protocol_R_choose, map_join_incl_compat.
-  - unfold node_entry.
-    etransitivity; [apply protocol_R_absorb; auto|].
-    view_shift_intros; reflexivity.
-Qed.
+(* up *)
+(* simple load_acq with read assertion *)
+Definition load_acq_witness {state} l (s : state) st_ord T P Q := (l, s, st_ord, T, protocol_R l s st_ord T * P,
+  fun _ : Z => FF, @nil Z, P, fun s' (v' : Z) => protocol_R l s' st_ord T * Q s' v').
 
-Corollary node_entry_choose : forall log1 log2 locs g lg i,
-  view_shift (node_entry Share.bot log1 locs g lg i * node_entry Share.bot log2 locs g lg i)
-    (node_entry Share.bot log1 locs g lg i).
-Proof.
-  intros; apply node_entry_absorb.
-Qed.
+(* simple load_acq with write assertion *)
+Definition load_acq_W_witness {state} l (s : state) st_ord T P Q := (l, s, st_ord, T, protocol_W l s st_ord T * P,
+  fun _ : Z => FF, @nil Z, protocol_W l s st_ord T * P,
+  fun s' (v' : Z) => !!(s' = s) && protocol_W l s st_ord T * Q s' v').
 
 Lemma body_read : semax_body Vprog Gprog f_read read_spec.
 Proof.
   start_atomic_function.
-  destruct x as ((((((((((n, out), sh), shi), version), locs), g), g'), lg), L0), v0); Intros.
+  destruct x as ((((((((n, out), sh), shi), version), locs), g), L0), v0); Intros.
   destruct H as (HP0 & HP & HQ).
   rewrite map_map in HP, HQ.
   assert (0 <= size) by (rewrite size_def; computable).
@@ -355,9 +413,10 @@ Proof.
   match goal with H : exists vs, _ |- _ => destruct H as [vs0 [? [HL0 ?]]] end.
   apply semax_pre with (P' := PROP () LOCAL (temp _n n; temp _out out)
     SEP (@data_at CompSpecs sh tnode (version, locs) n; data_at_ shi (tarray tint size) out;
-         EX v : Z, !!(v0 <= v) && protocol_R version g v Z.le (version_T locs g lg g');
-         EX ll : _, fold_right sepcon emp (map (fun i => node_entry Share.bot (Znth i ll empty_map) locs g lg i)
-           (upto (Z.to_nat size))); EX L' : _, ghost_snap (map_add L0 L') g';
+         EX v : Z, !!(v0 <= v) && protocol_R version v Z.le (version_T version locs g, version_T version locs g);
+         EX ll : _, fold_right sepcon emp (map (fun i =>
+           protocol_R (Znth i locs Vundef) (Znth i ll empty_map) map_incl (data_T version locs g, data_T version locs g)) (upto (Z.to_nat size)));
+         EX L' : _, ghost_snap (map_add L0 L') g;
          fold_right sepcon emp (map (fun p : Z => invariant (II p)) lI); P)).
   { unfold node_state; Intros.
     Exists v0 (map (fun i => map_Znth i L0 0) (upto (Z.to_nat size))) (@empty_map Z (list Z));
@@ -367,16 +426,17 @@ Proof.
   eapply semax_loop; [|forward; unfold loop2_ret_assert; apply drop_tc_environ].
   Intros v ll L'.
   repeat forward.
-  forward_call_dep [Z : Type] (version, g, v, Z.le, version_T locs g lg g', emp, version_T locs g lg g').
-  { split; intros; [|apply version_T_duplicable].
-    etransitivity; [apply view_shift_sepcon2, version_T_duplicable|].
-    rewrite <- sepcon_assoc; reflexivity. }
-  unfold version_T at 2; Intros x L1; destruct x as (v1', v1); simpl in *; subst.
+  forward_call_dep [Z : Type] (load_acq_witness version v Z.le
+    (version_T version locs g, version_T version locs g) emp (version_T version locs g)).
+  { simpl; cancel. }
+  { simpl; split; intros; rewrite ?emp_sepcon, ?sepcon_emp; try reflexivity.
+    rewrite sepcon_comm; reflexivity. }
+  Intro x; rewrite version_T_eq; Intros L1; destruct x as (v1', v1); simpl in *; subst.
   gather_SEP 7 3; rewrite map_snap_join; Intros.
   gather_SEP 3 6; rewrite <- sepcon_map; eapply view_shift_sepcon_list with (l2 := map _ (upto (Z.to_nat size)));
     rewrite ?Zlength_map; auto; intros.
   { erewrite !Znth_map, !Znth_upto by (auto; rewrite ?Zlength_upto in *; omega).
-    apply node_entry_choose. }
+    apply protocol_R_choose. }
   match goal with |-semax _ (PROP () (LOCALx ?Q (SEPx ?R))) _ _ =>
     forward_if (PROP (Z.even v1 = true) (LOCALx Q (SEPx R))) end.
   { eapply semax_pre; [|apply semax_continue].
@@ -401,12 +461,12 @@ Proof.
     SEP (@data_at CompSpecs sh tnode (version, locs) n;
          data_at shi (tarray tint size) (map (fun x => vint x) vals ++ repeat Vundef (Z.to_nat (size - i))) out;
          EX vers' : list Z, !!(Zlength vers' = i /\ Forall (fun v => Z.even v = true /\ v1 <= v) vers' /\
-             forall j, 0 <= j < i -> Znth j vers' 0 = v1 -> map_Znth j L1 0 v1 = Some (Znth j vals 0)) &&
-           protocol_R version g (list_max v1 (map (fun x => x - 1) vers')) Z.le (version_T locs g lg g') *
-           fold_right sepcon emp (map (fun i => node_entry Share.bot (singleton (Znth i vers' 0) (Znth i vals 0)) locs g lg i)
-             (sublist 0 i (upto (Z.to_nat size))));
-         fold_right sepcon emp (map (fun i => node_entry Share.bot (map_Znth i L1 0)
-           locs g lg i) (sublist i size (upto (Z.to_nat size)))); ghost_snap (map_add (map_add L0 L') L1) g';
+           forall j, 0 <= j < i -> forall v, map_Znth j L1 0 (Znth j vers' 0) = Some v -> v = Znth j vals 0) &&
+           protocol_R version (list_max v1 (map (fun x => x - 1) vers')) Z.le (version_T version locs g, version_T version locs g) *
+           fold_right sepcon emp (map (fun i => protocol_R (Znth i locs Vundef)
+             (singleton (Znth i vers' 0) (Znth i vals 0)) map_incl (data_T version locs g, data_T version locs g)) (sublist 0 i (upto (Z.to_nat size))));
+         fold_right sepcon emp (map (fun i => protocol_R (Znth i locs Vundef) (map_Znth i L1 0) map_incl
+           (data_T version locs g, data_T version locs g)) (sublist i size (upto (Z.to_nat size)))); ghost_snap (map_add (map_add L0 L') L1) g;
          fold_right sepcon emp (map (fun p : Z => invariant (II p)) lI); P)).
   { Exists (@nil Z) (@nil Z).
     rewrite data_at__eq; unfold default_val; simpl data_at.
@@ -421,27 +481,31 @@ Proof.
       eapply Forall_impl; [|eauto]; auto. }
     { rewrite <- size_def; apply prop_right; auto. }
     erewrite sublist_next with (i0 := i), Znth_upto by (rewrite ?Zlength_upto, ?Z2Nat.id; auto; omega); simpl.
-    forward_call_dep [Z -> option Z : Type] (Znth i locs Vundef, Znth i lg Vundef,
-      map_Znth i L1 0, @map_incl Z Z, data_T g,
-      protocol_R version g (list_max v1 (map (fun x => x - 1) vers')) Z.le (version_T locs g lg g'),
-      fun s (v : Z) => EX v' : Z, !!(Z.even v' = true /\ log_latest s v' v) &&
-        protocol_R version g (list_max v1 (map (fun x => x - 1) (vers' ++ [v']))) Z.le (version_T locs g lg g')).
-    { fast_cancel. }
-    { split; [|intros; apply exp_duplicable; intro; apply prop_duplicable, protocol_R_duplicable].
-      intros; unfold data_T.
+    forward_call_dep [Z -> option Z : Type] (load_acq_witness (Znth i locs Vundef) (map_Znth i L1 0) map_incl
+      (data_T version locs g, data_T version locs g)
+      (protocol_R version (list_max v1 (map (fun x0 : Z => x0 - 1) vers')) Z.le
+        (version_T version locs g, version_T version locs g))
+      (fun s (v : Z) => EX v' : Z, !!(Z.even v' = true /\ log_latest s v' v) &&
+        |>protocol_R version (list_max v1 (map (fun x => x - 1) (vers' ++ [v']))) Z.le (version_T version locs g, version_T version locs g))).
+    { simpl; cancel. }
+    { split; simpl; intros; rewrite !emp_sepcon; [reflexivity|].
+      rewrite data_T_eq.
       view_shift_intro ver; view_shift_intros.
-      etransitivity; [apply view_shift_sepcon1, protocol_R_duplicable|].
-      etransitivity; [apply view_shift_sepcon2, ghost_snap_duplicable|].
-      unfold protocol_R, protocol_piece at 2.
-      rewrite !sepcon_assoc, <- (sepcon_assoc (ghost _ _)); setoid_rewrite ghost_snap_join_Z.
-      rewrite <- !sepcon_assoc, (sepcon_assoc _ (invariant _)).
-      apply derives_view_shift; Exists ver ver; entailer!.
+      
+Axiom protocol_later : forall {state} sh l (s : state) ord Tread Tfull,
+  protocol_piece sh l s ord (|>Tread, |>Tfull) |-- |>protocol_piece sh l s ord (Tread, Tfull).
+
+      rewrite sepcon_comm, <- sepcon_assoc.
+      etransitivity; [apply view_shift_sepcon1, view_shift_sepcon;
+        apply derives_view_shift; [apply now_later | apply protocol_later]|].
+      rewrite <- later_sepcon; setoid_rewrite protocol_R_join; [|simpl; eauto].
+      apply derives_view_shift; Exists ver; entailer!.
+      apply later_derives.
       rewrite map_app, list_max_app; simpl.
       rewrite Z.max_comm, list_max_max; auto. }
     Intros y v'; destruct y as (d, log'); simpl in *.
-    eapply node_entry_single.
+    focus_SEP 1; eapply protocol_R_single.
     { match goal with H : log_latest _ _ _ |- _ => destruct H; eauto end. }
-    gather_SEP 1 2; rewrite protocol_R_R.
     forward.
     go_lower; Exists (x ++ [d]) (vers' ++ [v']); rewrite !Zlength_app, !Zlength_cons, !Zlength_nil.
     match goal with H : exists vs, _ /\ log_latest _ _ _ |- _ => destruct H as (vs1 & ? & HL1) end.
@@ -452,17 +516,14 @@ Proof.
         eapply log_incl_latest; eauto.
         unfold map_Znth, map_add.
         destruct HL1 as [->]; simpl; eauto.
-      + intros ?? Hj.
-        destruct (zlt j (Zlength x)); [assert (0 <= j < Zlength x) by tauto; rewrite app_Znth1 in * by omega; eauto|].
-        rewrite app_Znth2 in * by omega.
-        assert (j = Zlength x) by omega; subst j.
-        replace (Zlength vers') with (Zlength x) in Hj by omega;
-          rewrite Zminus_diag, Znth_0_cons in Hj |- *; subst.
-        assert (exists v, map_Znth (Zlength x) L1 0 v1 = Some v) as [d' Hd'].
-        { unfold map_Znth.
-          match goal with H : log_latest L1 _ _ |- _ => destruct H as [->]; simpl; eauto end. }
-        match goal with H : map_incl _ _ |- _ => pose proof (H _ _ Hd') as Hd'' end.
-        match goal with H : log_latest log' _ _ |- _ => destruct H as [Hd]; rewrite Hd in Hd''; inv Hd''; auto end. }
+      + intros ??? Hv.
+        destruct (eq_dec j (Zlength x)).
+        * subst; rewrite app_Znth2 in Hv |- * by omega.
+          replace (Zlength vers') with (Zlength x) in Hv; rewrite Zminus_diag, Znth_0_cons in Hv |- *.
+          match goal with H : map_incl _ log' |- _ => pose proof (H _ _ Hv) as Heq end.
+          match goal with H : log_latest log' _ _ |- _ => destruct H as [Hv']; rewrite Hv' in Heq end.
+          inv Heq; auto.
+        * rewrite app_Znth1 in Hv |- * by omega; match goal with H : forall j, _ |- _ => apply H; auto; omega end. }
     rewrite sublist_split with (mid := Zlength x)(hi := Zlength x + 1)
       by (rewrite ?Zlength_upto, ?Z2Nat.id; simpl; omega).
     erewrite sublist_len_1, Znth_upto by (rewrite ?Zlength_upto, ?Z2Nat.id; simpl; omega).
@@ -474,15 +535,16 @@ Proof.
     rewrite Zlength_sublist in Hi by (rewrite ?Zlength_upto, ?Z2Nat.id; simpl; omega).
     rewrite !Znth_sublist, !Znth_upto by (rewrite ?Z2Nat.id; simpl; omega).
     rewrite !app_Znth1 by omega; auto.
-    { rewrite map_app, list_max_app; simpl.
-      rewrite <- list_max_max; apply Z.le_max_r. }
   - Intros vals' vers'; rewrite <- size_def in *.
     rewrite Zminus_diag, app_nil_r, sublist_nil, sublist_same by (rewrite ?Zlength_upto, ?Z2Nat.id; auto).
-    forward_call_dep [Z : Type] (version, g, list_max v1 (map (fun x => x - 1) vers'), Z.le,
-      version_T locs g lg g', emp, fun s v : Z => !!(v = s) && emp).
-    { split; [|auto with dup].
-      intros; unfold version_T.
-      apply derives_view_shift; entailer!. }
+    forward_call_dep [Z : Type] (load_acq_witness version (list_max v1 (map (fun x => x - 1) vers')) Z.le
+      (version_T version locs g, version_T version locs g) emp (fun s v : Z => !!(v = s) && emp)).
+    { simpl; cancel. }
+    { simpl; split; intros; rewrite ?emp_sepcon, ?sepcon_emp; [reflexivity|].
+      rewrite version_T_eq; apply derives_view_shift; entailer!.
+      (* Iris assumes that anything duplicable has empty footprint, and anyway doesn't care about throwing away
+         resources. Should we make that assumption, or adjust the load rule? *)
+      admit. }
     Intros x; destruct x as (v2', v2); simpl in *; subst.
     match goal with |-semax _ (PROP () (LOCALx ?Q (SEPx ?R))) _ _ =>
       forward_if (PROP (v2 <> v1) (LOCALx Q (SEPx R))) end.
@@ -497,46 +559,41 @@ Proof.
         destruct (eq_dec (Znth j vers' 0) v1); subst; auto.
         assert (Znth j vers' 0 = v1 + 1) as Heq by omega.
         rewrite Heq, Z.even_add in Heven; replace (Z.even v1) with true in Heven; discriminate. }
-      assert (L1 v1 = Some vals') as HL1.
+      match goal with H : exists vs, _ |- _ => destruct H as [? [? [HL1]]] end.
+      assert (L1 v1 = Some vals') as Hvals'.
       { eapply map_Znth_eq.
-        * intros ? HL1.
-          match goal with H : exists vs, _ |- _ => destruct H as [? [? [Heq]]]; rewrite Heq in HL1; inv HL1; omega end.
+        * intro; rewrite HL1; intro X; inv X; omega.
         * intro; subst; rewrite size_def in *; discriminate.
-        * intros j Hj; replace (Zlength vals') with size in Hj; auto. }
-      gather_SEP 0 5 7 9 8; rewrite <- !sepcon_assoc; apply invariants_view_shift with
-        (Q0 := node_state Share.bot (singleton v1 vals') v1 version locs g lg g' * EX L : _, Q L (v1, vals')).
-      { rewrite !map_map, !sepcon_assoc, (sepcon_comm P), <- 2sepcon_assoc.
+        * intros; unfold map_Znth in *; rewrite HL1; simpl.
+          match goal with H : forall j, _ |- _ => apply f_equal, H; [omega|] end.
+          rewrite Hvers, HL1 by omega; auto. }
+      gather_SEP 6 8 7; rewrite <- !sepcon_assoc; apply invariants_view_shift with
+        (Q0 := ghost_snap (singleton v1 vals') g * EX L : _, Q L (v1, vals')).
+      { rewrite !map_map, !sepcon_assoc, (sepcon_comm P).
         etransitivity; [apply view_shift_sepcon2, HP|].
         view_shift_intro L2.
         etransitivity; [|apply derives_view_shift; Exists L2; apply derives_refl].
-        rewrite !sepcon_assoc, (sepcon_comm (Q _ _)).
+        rewrite (sepcon_comm (Q _ _)).
         etransitivity; [|apply view_shift_sepcon2, HQ]; simpl.
-        rewrite <- !sepcon_assoc, (sepcon_comm _ (ghost _ g')).
-        rewrite <- !sepcon_assoc, (sepcon_comm _ (ghost_snap _ g')).
-        rewrite <- !sepcon_assoc, snap_master_join by auto.
-        view_shift_intros.
-        rewrite !sepcon_assoc; etransitivity; [apply view_shift_sepcon1, make_snap|].
-        assert (L2 v1 = Some vals').
-        { match goal with H : map_incl _ _ |- _ => apply H end.
-          rewrite map_add_comm by auto.
-          unfold map_add; rewrite HL1; auto. }
-        assert (map_incl (singleton v1 vals') L2).
-        { unfold singleton; intros ??.
-          if_tac; [intro X; inv X; auto | discriminate]. }
-        rewrite !sepcon_assoc; etransitivity;
+        rewrite <- sepcon_assoc, snap_master_join by auto.
+        view_shift_intros; etransitivity; [apply view_shift_sepcon1, make_snap|].
+        match goal with H : map_incl _ L2 |- _ => exploit (H v1 vals') end.
+        { rewrite map_add_comm by auto.
+          unfold map_add; rewrite Hvals'; auto. }
+        rewrite sepcon_assoc; etransitivity;
           [apply view_shift_sepcon1, ghost_snap_forget with (v2 := singleton v1 vals'); auto|].
-        { intros; eapply map_join_incl_compat; eauto. }
-        apply derives_view_shift; unfold node_state, protocol_R, ghost_snap, share; entailer!.
-        { exists vals'; split; auto.
-          apply log_latest_singleton. }
-        erewrite map_ext_in; eauto; intros; simpl.
-        rewrite map_Znth_single, Hvers; auto.
-        rewrite In_upto, Z2Nat.id in *; auto. }
+        { intros ??; unfold singleton; if_tac; intro X; inv X; auto. }
+        apply derives_view_shift; entailer!. }
       Intros L2.
       forward.
-      rewrite map_map; Exists (v1, vals') L2; entailer!.
-      rewrite HL0; match goal with H : compatible _ _ |- _ => eapply f_equal, H; eauto end.
-      unfold map_add; rewrite HL0; auto.
+      rewrite map_map; Exists (v1, vals') L2; unfold node_state, protocol_R, ghost_snap, share; entailer!.
+      { split.
+        * intro; subst; rewrite HL0; match goal with H : compatible _ _ |- _ => eapply f_equal, H; eauto end.
+          unfold map_add; rewrite HL0; auto.
+        * do 2 eexists; [|apply log_latest_singleton]; auto. }
+      erewrite map_ext_in; eauto; intros; simpl.
+      rewrite map_Znth_single, Hvers; auto.
+      rewrite In_upto, Z2Nat.id in *; auto.
     + forward.
       entailer!.
     + intros; unfold overridePost.
@@ -547,43 +604,45 @@ Proof.
       { destruct (list_max_spec (map (fun x => x - 1) vers') v1); omega. }
       erewrite map_ext_in; eauto; intros; simpl.
       rewrite In_upto in *; erewrite Znth_map, Znth_upto; rewrite ?Zlength_upto; auto; omega.
-Qed.
+Admitted.
+
+(* simple store_rel recovering write assertion *)
+Definition store_rel_witness {state} l (v : Z) (s s'' : state) st_ord T P Q := (l, v, s, s'', st_ord, T,
+  protocol_W l s st_ord T * P, fun _ : Z => FF, @nil Z, P, protocol_W l s'' st_ord T * Q).
 
 (* Is there any use to allowing RA atomics to interact with invariants if they can't take or leave protocol
    assertions? Possibly. *)
+(* Since the public view of the data structure has no data content (it's just the ghost state), there's no need
+   for the backing-out linearization point reasoning (and in fact the linearization point can be anywhere,
+   since all new write really guarantees is that no other data will be written at that version, plus maybe a
+   certain eventual consistency). *)
 Lemma body_write : semax_body Vprog Gprog f_write write_spec.
 Proof.
   start_atomic_function.
-  destruct x as (((((((((((n, input), sh), shi), version), locs), vals), g), g'), lg), L), v0); Intros.
+  destruct x as (((((((((n, input), sh), shi), version), locs), vals), g), L), v0); Intros.
   destruct H as (HP0 & HP & HQ).
   forward.
   rewrite map_map in HP, HQ.
   unfold node_state; Intros.
-  focus_SEP 2; apply make_protocol_R.
-  forward_call_dep [Z : Type] (version, g, v0, Z.le, version_T locs g lg g',
-    protocol_piece gsh2 version g v0 Z.le (version_T locs g lg g'), fun s v : Z => !!(v = s) && emp).
-  { split; [|auto with dup].
-    intros.
-    apply derives_view_shift; unfold version_T; entailer!. }
+  forward_call_dep [Z : Type] (load_acq_W_witness version v0 Z.le (version_T version locs g, version_T version locs g)
+    emp (fun s v : Z => !!(v = s) && emp)).
+  { simpl; unfold protocol_W; cancel. }
+  { simpl; split; intros; rewrite !emp_sepcon, !sepcon_emp.
+    { rewrite sepcon_comm; apply make_protocol_R. }
+    rewrite sepcon_assoc; etransitivity;
+      [apply view_shift_sepcon2; rewrite sepcon_comm; apply protocol_R_absorb; auto|].
+    view_shift_intros; assert (s' = v0) by omega.
+    apply derives_view_shift; rewrite version_T_eq; unfold protocol_W; entailer!.
+    admit. (* as above *) }
   Intros x; destruct x as (?, v); simpl in *; subst.
-  gather_SEP 1 0; apply protocol_R_absorb; auto; Intros.
-  assert (v = v0) by omega; subst.
   assert (repable_signed (v0 + 1)) by admit. (* version stays in range *)
-  forward_call_dep [Z : Type] (version, v0 + 1, g, v0, v0 + 1, Z.le, version_T locs g lg g',
-    P * protocol_piece gsh2 version g v0 Z.le (version_T locs g lg g'), II, lI,
-    EX L : _, ghost (gsh1, L) g' * R L,
-    P * protocol_piece gsh2 version g (v0 + 1) Z.le (version_T locs g lg g')).
-  { split; [auto | split; [|split; [|omega]]].
-    - rewrite <- sepcon_assoc; etransitivity; [apply view_shift_sepcon1, HP|].
-      rewrite sepcon_comm; reflexivity.
-    - intros.
-      rewrite <- !sepcon_assoc, (sepcon_comm _ (protocol_piece _ _ _ _ _ _)), <- !sepcon_assoc, (sepcon_assoc _ _ P).
-      etransitivity; [|apply view_shift_sepcon2, HP].
-      unfold version_T at 1 4.
-      view_shift_intro L0; view_shift_intro L1; view_shift_intros.
-      apply derives_view_shift.
-      Exists L0 L1; entailer!.
-      rewrite Z.even_add, Z.add_simpl_r; replace (Z.even v0) with true in *; auto. }
+  forward_call_dep [Z : Type] (store_rel_witness version (v0 + 1) v0 (v0 + 1) Z.le
+    (version_T version locs g, version_T version locs g) emp emp).
+  { simpl; cancel. }
+  { split; auto; split; [|split; [|omega]]; intros; simpl; rewrite !sepcon_emp, ?emp_sepcon; [reflexivity|].
+    rewrite !version_T_eq.
+    apply derives_view_shift; Intros L1; Exists L1.
+    subst; rewrite Z.even_add, Z.add_simpl_r, H in *; simpl; entailer!. }
   assert (0 <= size) by (rewrite size_def; computable).
   assert_PROP (Zlength (map (fun x => vint x) vals) = size) by entailer!.
   assert (Z.even (v0 + 2) = true) by (rewrite Z.even_add; replace (Z.even v0) with true; auto).
@@ -591,10 +650,12 @@ Proof.
   focus_SEP 4.
   match goal with |-semax _ (PROP () (LOCALx ?Q (SEPx (_ :: ?R)))) _ _ =>
   forward_for_simple_bound 8 (EX i : Z, PROP () (LOCALx Q
-    (SEPx (fold_right sepcon emp (map (fun i => node_entry gsh2 (map_Znth i (map_upd L (v0 + 2) vals) 0)
-             locs g lg i) (sublist 0 i (upto (Z.to_nat size)))) ::
-           fold_right sepcon emp (map (fun i => node_entry gsh2 (map_Znth i L 0)
-             locs g lg i) (sublist i size (upto (Z.to_nat size)))) :: R)))) end.
+    (SEPx (fold_right sepcon emp (map (fun i => protocol_W (Znth i locs Vundef)
+             (map_Znth i (map_upd L (v0 + 2) vals) 0) map_incl (data_T version locs g, data_T version locs g))
+             (sublist 0 i (upto (Z.to_nat size)))) ::
+           fold_right sepcon emp (map (fun i => protocol_W (Znth i locs Vundef)
+             (map_Znth i L 0) map_incl (data_T version locs g, data_T version locs g))
+             (sublist i size (upto (Z.to_nat size)))) :: R)))) end.
   { rewrite sublist_nil, sublist_same by (rewrite ?Zlength_upto, ?Z2Nat.id; auto).
     replace (Z.even v0) with true; entailer!. }
   - (* loop body *)
@@ -608,89 +669,59 @@ Proof.
     match goal with H : exists vs, _ |- _ => destruct H as [vs0 [? ?]] end.
     destruct (log_latest_upd (map_Znth i L 0) v0 (Znth i vs0 0) (v0 + 2) (Znth i vals 0)); auto; try omega.
     { apply map_Znth_log_latest; auto. }
-    unfold node_entry at 2.
-    forward_call_dep [Z -> option Z : Type] (Znth i locs Vundef, Znth i vals 0, Znth i lg Vundef,
-      map_Znth i L 0, map_upd (map_Znth i L 0) (v0 + 2) (Znth i vals 0), @map_incl Z Z, data_T g,
-      P * protocol_piece gsh2 version g (v0 + 1) Z.le (version_T locs g lg g') *
-        protocol_piece gsh2 (Znth i locs Vundef) (Znth i lg Vundef) (map_Znth i L 0) map_incl (data_T g) *
-        ghost (gsh2, L) g', II, lI,
-      !!(exists vs, Zlength vs = size /\ log_latest L v0 vs) &&
-        protocol_piece gsh2 version g (v0 + 1) Z.le (version_T locs g lg g') *
-        ghost (gsh1, L) g' * ghost (gsh2, L) g' * R L,
-      P * protocol_piece gsh2 version g (v0 + 1) Z.le (version_T locs g lg g') *
-        protocol_piece gsh2 (Znth i locs Vundef) (Znth i lg Vundef) (map_Znth i (map_upd L (v0 + 2) vals) 0)
-          map_incl (data_T g) * ghost (gsh2, L) g').
-    { fast_cancel. }
+    forward_call_dep [Z -> option Z : Type] (store_rel_witness (Znth i locs Vundef) (Znth i vals 0)
+      (map_Znth i L 0) (map_upd (map_Znth i L 0) (v0 + 2) (Znth i vals 0)) map_incl (data_T version locs g, data_T version locs g)
+      (protocol_W version (v0 + 1) Z.le (version_T version locs g, version_T version locs g))
+      (protocol_W version (v0 + 1) Z.le (version_T version locs g, version_T version locs g))).
+    { simpl; cancel. }
     { split; [apply Forall_Znth; auto; omega|].
       assert (0 <= i < Zlength (upto (Z.to_nat size))) by (rewrite Zlength_upto, Z2Nat.id; auto; omega).
-      split; [|split; auto].
-      + rewrite <- !sepcon_assoc, 2sepcon_assoc; etransitivity; [apply view_shift_sepcon1, HP|].
-        unfold node_state.
-        view_shift_intro L1; view_shift_intro v; view_shift_intros.
-        apply view_shift_assert with (PP := L1 = L); [|intro; subst].
-        { rewrite (sepcon_comm _ (ghost _ _)), <- !sepcon_assoc, (sepcon_comm _ (ghost _ _)).
-          rewrite <- !sepcon_assoc; do 3 apply sepcon_derives_prop.
-          rewrite sepcon_comm; setoid_rewrite ghost_var_share_join'; eauto; entailer!. }
-        apply derives_view_shift; entailer!.
-        eauto.
-      + intros.
-        rewrite !sepcon_assoc, (sepcon_comm (data_T _ _ (Znth i vals 0))).
-        rewrite <- 5sepcon_assoc; etransitivity; [|apply view_shift_sepcon1, view_shift_sepcon1, HP].
-        unfold data_T at 1 4.
-        view_shift_intro ver; view_shift_intros.
-        rewrite <- !sepcon_assoc, (sepcon_comm _ (protocol_piece _ version _ _ _ _)).
-        rewrite <- sepcon_assoc.
-        rewrite 3sepcon_assoc; etransitivity; [apply view_shift_sepcon1 with (P' :=
-          !!(ver - 1 <= v0 + 1) && protocol_piece gsh2 version g (v0 + 1) Z.le (version_T locs g lg g') *
-          ghost_snap (v0 + 1) g)|].
-        { unfold protocol_piece.
-          rewrite sepcon_assoc, (sepcon_comm (ghost _ _)), snap_master_join by auto.
-          view_shift_intros; etransitivity; [apply view_shift_sepcon2, make_snap|].
-          apply derives_view_shift; entailer!. }
-        view_shift_intros.
-        apply derives_view_shift.
-        Exists L (v0 + 2).
-        rewrite map_Znth_upd, <- Z.add_sub_assoc; simpl.
-        entailer!. }
+      split; [|split; auto]; intros; simpl; rewrite ?emp_sepcon, ?sepcon_emp; [reflexivity|].
+      rewrite !data_T_eq; view_shift_intro ver; view_shift_intros.
+      rewrite sepcon_comm; etransitivity; [apply view_shift_sepcon1, make_protocol_R|].
+      apply derives_view_shift; Exists (v0 + 2).
+      rewrite <- Z.add_sub_assoc; simpl; unfold protocol_W; entailer!.
+
+Axiom protocol_delay : forall {state} sh l (s : state) ord Tread Tfull,
+  protocol_piece sh l s ord (Tread, Tfull) |-- protocol_piece sh l s ord (|>Tread, |>Tfull).
+
+      eapply derives_trans; [apply sepcon_derives, derives_refl; apply protocol_delay|].
+      simpl; unfold protocol_R; cancel.
+      admit. (* as above *) }
     erewrite sublist_split with (mid := i)(hi := i + 1), sublist_len_1, Znth_upto, map_app, sepcon_app
       by (rewrite ?Zlength_upto, ?Z2Nat.id; auto; omega); simpl fold_right.
-    rewrite <- size_def; unfold node_entry; entailer!.
+    rewrite <- size_def, map_Znth_upd; entailer!.
   - rewrite <- size_def, sublist_nil, sublist_same by (rewrite ?Zlength_upto, ?Z2Nat.id; auto; omega).
     assert (repable_signed (v0 + 2)) by admit.
     match goal with H : exists vs, _ |- _ => destruct H as [vs0 [? ?]] end.
     destruct (log_latest_upd L v0 vs0 (v0 + 2) vals); auto; try omega.
-    forward_call_dep [Z : Type] (version, v0 + 2, g, v0 + 1, v0 + 2, Z.le, version_T locs g lg g',
-      P * protocol_W version g (v0 + 1) Z.le (version_T locs g lg g') *
-        fold_right sepcon emp (map (fun i => node_entry gsh2 (map_Znth i (map_upd L (v0 + 2) vals) 0)
-          locs g lg i) (upto (Z.to_nat size))) * ghost (gsh2, L) g', II, lI,
-      !!(exists vs, Zlength vs = size /\ log_latest L v0 vs) &&
-        fold_right sepcon emp (map (fun i => node_entry gsh2 (map_Znth i (map_upd L (v0 + 2) vals) 0)
-          locs g lg i) (upto (Z.to_nat size))) * ghost (Tsh, L) g' * R L,
-      Q L tt * protocol_W version g (v0 + 2) Z.le (version_T locs g lg g') *
-        fold_right sepcon emp (map (fun i => node_entry gsh2 (map_Znth i (map_upd L (v0 + 2) vals) 0)
-          locs g lg i) (upto (Z.to_nat size))) * ghost (gsh2, map_upd L (v0 + 2) vals) g').
+    forward_call_dep [Z : Type] (version, v0 + 2, v0 + 1, v0 + 2, Z.le, (version_T version locs g, version_T version locs g),
+      P * protocol_W version (v0 + 1) Z.le (version_T version locs g, version_T version locs g) *
+        fold_right sepcon emp (map (fun i => protocol_W (Znth i locs Vundef) (map_Znth i (map_upd L (v0 + 2) vals) 0)
+          map_incl (data_T version locs g, data_T version locs g)) (upto (Z.to_nat size))) * ghost (gsh2, L) g, II, lI,
+      fold_right sepcon emp (map (fun i => protocol_W (Znth i locs Vundef) (map_Znth i (map_upd L (v0 + 2) vals) 0)
+          map_incl (data_T version locs g, data_T version locs g)) (upto (Z.to_nat size))) * ghost (Tsh, L) g * R L,
+      Q L tt * node_state gsh2 (map_upd L (v0 + 2) vals) (v0 + 2) version locs g).
     { fast_cancel. }
     { split; [auto | split; [| split; [|omega]]].
       + rewrite <- !sepcon_assoc, 2sepcon_assoc; etransitivity; [apply view_shift_sepcon1, HP|].
-        view_shift_intro L1; view_shift_intro v; unfold node_state.
-        view_shift_intros.
+        view_shift_intro L1.
         rewrite <- !sepcon_assoc, (sepcon_comm _ (ghost _ _)), <- !sepcon_assoc.
         rewrite (sepcon_comm (ghost _ _)); setoid_rewrite ghost_var_share_join'; eauto.
         apply derives_view_shift; entailer!.
-        eauto.
-      + intros.
-        rewrite !sepcon_assoc, (sepcon_comm (version_T _ _ _ _ (v0 + 2) _)).
-        rewrite <- !sepcon_assoc, 6sepcon_assoc.
+      + intros; simpl.
+        rewrite !sepcon_assoc, (sepcon_comm (version_T _ _ _ (v0 + 2) _)).
+        rewrite <- !sepcon_assoc, 4sepcon_assoc.
         etransitivity; [|apply view_shift_sepcon1, HQ].
-        unfold version_T at 1 4.
-        view_shift_intro L'; view_shift_intros.
+        rewrite !version_T_eq; view_shift_intro L'; view_shift_intros.
         rewrite <- !sepcon_assoc, (sepcon_comm _ (fold_right _ _ _)).
         rewrite <- !sepcon_assoc, <- sepcon_map.
         rewrite !sepcon_assoc; etransitivity; [apply view_shift_sepcon1, view_shift_sepcon_list|].
         { rewrite 2Zlength_map; reflexivity. }
         { rewrite Zlength_map; intros.
           erewrite !Znth_map, !Znth_upto by (auto; rewrite Zlength_upto in *; omega).
-          etransitivity; [apply node_entry_absorb | apply node_entry_snap]. }
+          etransitivity; [apply protocol_R_absorb; auto|].
+          apply view_shift_prop; intro; apply make_protocol_R. }
         rewrite <- !sepcon_assoc, (sepcon_comm _ (ghost _ _)).
         rewrite <- !sepcon_assoc, (sepcon_comm _ (ghost_snap _ _)).
         rewrite <- !sepcon_assoc, snap_master_join by apply Share.nontrivial; view_shift_intros.
@@ -698,16 +729,27 @@ Proof.
         { apply view_shift_sepcon1; etransitivity.
           * apply master_update with (v' := map_upd L (v0 + 2) vals); auto.
           * apply make_snap. }
-        fold (ghost_var Tsh (map_upd L (v0 + 2) vals) g').
+        fold (ghost_var Tsh (map_upd L (v0 + 2) vals) g).
         erewrite <- ghost_var_share_join by eauto.
         apply derives_view_shift; Exists (map_upd L (v0 + 2) vals).
         rewrite Zlength_map in *; rewrite sepcon_map.
         rewrite Z.even_add; replace (Z.even v0) with true; simpl.
-        unfold ghost_var; entailer!; eauto. }
+        unfold ghost_var, node_state; entailer!.
+        split; eauto. }
     forward.
-    Exists tt L; unfold node_state.
-    rewrite Zlength_map in *; unfold protocol_W; entailer!; eauto.
+    Exists tt L.
+    rewrite Zlength_map in *; entailer!.
 Admitted.
+
+(* up *)
+Lemma list_duplicate : forall Q lP, duplicable Q ->
+  view_shift (fold_right sepcon emp lP * Q) (fold_right sepcon emp (map (sepcon Q) lP) * Q).
+Proof.
+  induction lP; simpl; intros; [reflexivity|].
+  rewrite sepcon_assoc; etransitivity; [apply view_shift_sepcon2, IHlP; auto|].
+  rewrite <- sepcon_assoc; etransitivity; [apply view_shift_sepcon2, H|].
+  apply derives_view_shift; cancel.
+Qed.
 
 Lemma body_make_node : semax_body Vprog Gprog f_make_node make_node_spec.
 Proof.
@@ -715,74 +757,59 @@ Proof.
   forward_malloc tnode n.
   forward_malloc tint p.
   repeat forward.
-  apply ghost_alloc with (g := (Tsh, 0)); [apply master_init | Intros g].
-  apply make_snap; Intros.
-  apply ghost_snap_le with (v1 := -1); [omega|].
   forward_for_simple_bound 8 (EX i : Z, EX ld : list val, PROP (Zlength ld = i; Forall isptr ld)
     LOCAL (temp _n n)
-    SEP (ghost_snap (-1) g; ghost (Tsh, 0) g; malloc_token Tsh (sizeof tint) p; data_at Tsh tint (vint 0) p;
-         malloc_token Tsh (sizeof tnode) n;
+    SEP (malloc_token Tsh (sizeof tint) p; data_at Tsh tint (vint 0) p; malloc_token Tsh (sizeof tnode) n;
          @data_at CompSpecs Tsh tnode (p, ld ++ repeat Vundef (Z.to_nat (8 - i))) n;
-         EX lg : list val, !!(Zlength lg = i) && fold_right sepcon emp (map (fun i =>
-           node_entry gsh2 (singleton 0 0) ld g lg i *
-           node_entry Share.bot (singleton 0 0) ld g lg i) (upto (Z.to_nat i)));
+         fold_right sepcon emp (map (data_at Tsh tint (vint 0)) ld);
          fold_right sepcon emp (map (malloc_token Tsh (sizeof tint)) ld))).
-  { Exists (@nil val) (@nil val); entailer!; auto. }
-  - apply ghost_snap_duplicable.
-    Intros lg.
-    rewrite sepcon_map.
-    forward_malloc tint d.
+  { Exists (@nil val); entailer!; auto. }
+  - forward_malloc tint d.
     rewrite data_at__isptr; Intros.
-    forward.
-    gather_SEP 1 2; eapply view_shift_trans; [|apply (make_protocol d 0 (singleton 0 0) (data_T g)); auto|].
-    { unfold data_T.
-      apply derives_view_shift; Exists 0; entailer!.
-      apply log_latest_singleton. }
-    Intros gi.
-    replace_SEP 0 (node_entry gsh2 (singleton 0 0) (x ++ [d]) g (lg ++ [gi]) i).
-    { go_lower; unfold node_entry.
-      rewrite !app_Znth2 by omega.
-      replace (Zlength x) with i; replace (Zlength lg) with i; rewrite Zminus_diag, !Znth_0_cons; entailer!. }
-    apply node_entry_snap.
-    Intros; forward.
-    Exists (x ++ [d]) (lg ++ [gi]); rewrite upd_init, <- app_assoc, !Zlength_app, !Zlength_cons,
-      !Zlength_nil by (auto; tauto).
-    rewrite Z2Nat.inj_add, upto_app, !map_app, !sepcon_app, Z2Nat.id by omega.
-    simpl fold_right.
-    rewrite Z.add_0_r; entailer!.
+    repeat forward.
+    Exists (x ++ [d]); rewrite upd_init, <- app_assoc, !Zlength_app, !Zlength_cons, !Zlength_nil by (auto; tauto).
+    rewrite !map_app, !sepcon_app; simpl fold_right; entailer!.
     { rewrite Forall_app; repeat constructor; auto. }
-    cancel; erewrite <- sepcon_map, map_ext_in; eauto; simpl; intros.
-    unfold node_entry.
-    rewrite In_upto, <- Zlength_correct in *.
-    rewrite !app_Znth1 by omega; auto.
-  - Intros ld lg.
-    rewrite <- size_def in *.
-    rewrite Zminus_diag, app_nil_r.
-    gather_SEP 0 1; rewrite snap_master_join by apply Share.nontrivial.
-    rewrite sepcon_map; Intros.
-    apply ghost_alloc with (g0 := (Tsh, singleton 0 (repeat 0 (Z.to_nat size))));
-      [apply master_init | Intros g'].
+    auto.
+  - Intros ld.
+    (* Initializing the mutually recursive protocols is hard. The best way is probably to say that version_T
+       doesn't need the snapshots if it's at version 0. *)
+    apply ghost_alloc with (g := (Tsh, singleton 0 (repeat 0 (Z.to_nat size))));
+      [apply master_init | Intros g].
     apply make_snap; Intros.
-    gather_SEP 4 2 8 0; eapply view_shift_trans;
-      [|apply (make_protocol'(ord := Z.le) p g 0 0 (version_T ld g lg g')); auto|].
-    { unfold version_T.
-      apply derives_view_shift; Exists (singleton 0 (repeat 0 (Z.to_nat size))); simpl.
-      unfold ghost_master; entailer!.
-      { do 2 eexists; [|apply log_latest_singleton].
-        rewrite Zlength_repeat, Z2Nat.id; auto; rewrite size_def; computable. }
-      erewrite map_ext; eauto; intros; simpl.
-      rewrite map_Znth_single, Znth_repeat; auto. }
-    forward.
-    fold (ghost_var Tsh (singleton 0 (repeat 0 (Z.to_nat size))) g');
-      erewrite <- ghost_var_share_join by eauto.
-    unfold node_state.
-    Exists n p ld g lg g'; unfold protocol_W, ghost_var; simpl; entailer!.
+    assert (exists vs, Zlength vs = size /\ log_latest (singleton 0 (repeat 0 (Z.to_nat size))) 0 vs).
     { do 2 eexists; [|apply log_latest_singleton].
       rewrite Zlength_repeat, Z2Nat.id; auto; rewrite size_def; computable. }
-    rewrite sepcon_comm; apply sepcon_derives; auto.
-    erewrite map_ext; eauto; simpl; intros.
+    gather_SEP 3 0; eapply view_shift_trans;
+      [|apply (@make_protocol _ _ Z.le _ _ (version_prot p ld g) p 0 0); auto|].
+    { rewrite version_T_eq; apply derives_view_shift.
+      Exists (singleton 0 (repeat 0 (Z.to_nat size))); simpl; entailer!.
+      admit. }
+    apply make_protocol_R; Intros.
+    focus_SEP 1; apply protocol_R_forget with (s1 := -1); [omega|].
+    rewrite app_nil_r; gather_SEP 6 0; apply list_duplicate.
+    { apply protocol_R_duplicable. }
+    Intros; apply view_shift_sepcon_list with (l2 := map (fun l =>
+      protocol_W l (singleton 0 0) map_incl (data_T p ld g, data_T p ld g)) ld); rewrite ?Zlength_map; auto.
+    { intros.
+      erewrite Znth_map, Znth_map', Znth_map with (d' := Vundef) by (rewrite ?Zlength_map; auto).
+      rewrite sepcon_comm; etransitivity; [|apply make_protocol with (v := 0); auto; apply data_prot].
+      rewrite data_T_eq.
+      apply derives_view_shift; Exists 0; entailer!.
+      { apply log_latest_singleton. }
+      simpl; apply protocol_delay. }
+    gather_SEP 2 1; apply protocol_R_absorb; auto; Intros.
+    forward.
+    fold (ghost_var Tsh (singleton 0 (repeat 0 (Z.to_nat size))) g);
+      erewrite <- ghost_var_share_join by eauto.
+    unfold node_state.
+    rewrite <- size_def in *.
+    Exists n p ld g; unfold protocol_W, ghost_var, share; simpl; entailer!.
+    setoid_rewrite (list_Znth_eq Vundef ld) at 3.
+    rewrite map_map, <- ZtoNat_Zlength; replace (Zlength ld) with size.
+    erewrite map_ext_in; eauto; intros; simpl.
     rewrite map_Znth_single, Znth_repeat; auto.
-Qed.
+Admitted.
 
 Lemma body_writer : semax_body Vprog Gprog f_writer writer_spec.
 Proof.
@@ -794,8 +821,8 @@ Proof.
     PROP (L' = map_upd_list L (map (fun i => (v + 2 * (i + 1), repeat (i + 1) 8)%Z) (upto (Z.to_nat i))))
     LOCAL (lvar _data (tarray tint 8) data; temp _n n)
     SEP (data_at Tsh (tarray tint 8) (repeat (vint i) 8) data; @data_at CompSpecs sh tnode (version, locs) n;
-         node_state gsh2 L' (v + 2 * i) version locs g lg g';
-         invariant (EX L : Z -> option (list Z), ghost (gsh1, L) g'))).
+         node_state gsh2 L' (v + 2 * i) version locs g;
+         invariant (EX L : Z -> option (list Z), ghost (gsh1, L) g))).
   { Exists L; entailer!; auto. }
   - Intros.
     match goal with |-semax _ (PROP () (LOCALx ?Q (SEPx (_ :: ?R)))) _ _ =>
@@ -833,9 +860,9 @@ Ltac lookup_spec_and_change_compspecs CS id ::=
    end)
  else elimtype  (Cannot_find_function_spec_in_Delta id).
 
-      forward_call (n, data, sh, Tsh, version, locs, repeat (i + 1) 8, g, g', lg, x, v + 2 * i, emp,
+      forward_call (n, data, sh, Tsh, version, locs, repeat (i + 1) 8, g, x, v + 2 * i, emp,
         fun (_ : Z -> option (list Z)) (_ : unit) => emp, fun _ : Z -> option (list Z) => emp,
-        fun _ : Z => EX L : Z -> option (list Z), ghost (gsh1, L) g', [0]).
+        fun _ : Z => EX L : Z -> option (list Z), ghost (gsh1, L) g, [0]).
       { entailer!.
         { apply Forall_repeat.
           split; [pose proof Int.min_signed_neg; omega|].
@@ -911,7 +938,7 @@ Proof.
       (* This also fails: the history in the invariant may not have caught up with the value we read. *)
 Abort.*)
 
-Lemma node_state_forget : forall L v version locs g lg g' L' v' (HL' : map_incl L' L) (Hv : v' <= v)
+(*Lemma node_state_forget : forall L v version locs g lg g' L' v' (HL' : map_incl L' L) (Hv : v' <= v)
   (Hv' : exists vs, Zlength vs = size /\ log_latest L' v' vs) (Heven : Z.even v' = true),
   view_shift (node_state Share.bot L v version locs g lg g')
              (node_state Share.bot L' v' version locs g lg g').
@@ -932,32 +959,23 @@ Proof.
     { intros; eapply map_join_incl_compat; eauto. }
     { transitivity (map_Znth i L 0); [|destruct (Z.even v); auto; subst; reflexivity].
       apply map_incl_Znth; auto. }
-Qed.
+Qed.*)
 
 (* up *)
-Lemma map_add_single : forall {A B} {A_eq : EqDec A} (m : A -> option B) k v, map_add (singleton k v) m = map_upd m k v.
+Lemma map_add_single : forall {A B} {A_eq : EqDec A} (m : A -> option B) k v,
+  map_add (singleton k v) m = map_upd m k v.
 Proof.
   intros; extensionality; unfold map_add, singleton, map_upd; if_tac; auto.
 Qed.
 
-Lemma node_entry_join : forall log1 log2 locs g lg i,
-  node_entry Share.bot log1 locs g lg i * node_entry Share.bot log2 locs g lg i |--
-  node_entry Share.bot (map_add log1 log2) locs g lg i.
-Proof.
-  intros; unfold node_entry.
-  eapply derives_trans; [apply protocol_R_join'|].
-  Intros log'.
-  match goal with H : join _ _ _ |- _ => rewrite map_join_spec in H; destruct H as [Hcompat]; subst; auto end.
-Qed.
-
-Lemma node_state_upd : forall L v v' vs' version locs g lg g' (Hv' : v <= v') (Hvs' : Zlength vs' = size)
+Lemma node_state_upd : forall L v v' vs' version locs g (Hv' : v <= v') (Hvs' : Zlength vs' = size)
   (Hcompat : v' = v -> L v' = Some vs'),
-  node_state Share.bot (singleton v' vs') v' version locs g lg g' *
-  node_state Share.bot L v version locs g lg g' |--
-  node_state Share.bot (map_upd L v' vs') v' version locs g lg g'.
+  node_state Share.bot (singleton v' vs') v' version locs g *
+  node_state Share.bot L v version locs g |--
+  node_state Share.bot (map_upd L v' vs') v' version locs g.
 Proof.
   intros; unfold node_state; Intros.
-  rewrite <- !sepcon_assoc, (sepcon_comm _ (protocol_piece _ _ _ _ _ _)).
+  rewrite <- !sepcon_assoc, (sepcon_comm _ (protocol_piece _ _ _ _ _)).
   rewrite <- !sepcon_assoc, 3sepcon_assoc.
   eapply derives_trans; [apply sepcon_derives, derives_refl; apply protocol_R_join'|].
   Intros v''.
@@ -973,7 +991,9 @@ Proof.
   { rewrite 2Zlength_map; reflexivity. }
   { rewrite Zlength_map; intros.
     erewrite !Znth_map, !Znth_upto by (auto; rewrite Zlength_upto in *; omega).
-    eapply derives_trans; [apply node_entry_join|].
+    eapply derives_trans; [apply protocol_R_join'|].
+    Intros log'.
+    match goal with H : join _ _ _ |- _ => rewrite map_join_spec in H; destruct H; subst end.
     rewrite <- map_Znth_add, map_add_single; apply derives_refl. }
   unfold ghost_snap, protocol_R; entailer!.
   destruct (eq_dec v' v).
@@ -991,10 +1011,10 @@ Proof.
   { unfold node_state; entailer!. }
   destruct Hv as [Heven [? [? [HL ?]]]].
   focus_SEP 2; apply node_state_snap.
-  forward_call (n, data, sh, Tsh, version, locs, g, g', lg, L, v, emp,
+  forward_call (n, data, sh, Tsh, version, locs, g, L, v, emp,
     fun (L' : Z -> option (list Z)) (_ : Z * list Z) => emp,
     fun _ : Z -> option (list Z) => emp,
-    fun _ : Z => EX L : Z -> option (list Z), ghost (gsh1, L) g', [0]).
+    fun _ : Z => EX L : Z -> option (list Z), ghost (gsh1, L) g, [0]).
   { rewrite <- size_def; simpl; entailer!. }
   { split; [|split].
     * admit.
@@ -1007,4 +1027,4 @@ Proof.
   forward.
   Exists data v' vs'; rewrite size_def; entailer!.
   apply node_state_upd; auto.
-Qed.
+Admitted.
